---
tags:
  - university-notes
university-name: Virtual University of Pakistan
date: 2025-04-08
---

# Lecture No. 18

<span style="color: gray;">Dated: 08-04-2025</span>

Here is the algorithm for computing the `FIRST sets`.[^1]

- For all `terminal` symbols $b$.  

$$\text{FIRST}(b) = \{b\}$$

- For all `productions` $X \to A_1 \ldots A_n$ or in general, $X \to A_i$.  

$$\text{Add FIRST}(A_i) - \{\epsilon\} \text{ to FIRST} (X) \text{, stop if } \epsilon \notin \text{FIRST}(A_i)$$

This strategy is encoded in the following procedure

for each $a \in (T \cup \epsilon)$ $\text{FIRST}(a) \to \{a\}$  
for each $A \in NT$ $\text{FIRST}(A) \to \emptyset$  
while (`FIRST sets`[^1] are still changing)  
	for each $A \to \beta_1 \beta_2 \ldots \beta_k \in P$  
		$\text{FIRST}(A) \to \text{FIRST}(A) \cup (\text{FIRST}(\beta_1) - \epsilon)$  
		$i \to 1$  
		while ($\epsilon \in \text{FIRST}(\beta_i)$ and $i = k - 1$)  
			$\text{FIRST}(A) \to \text{FIRST}(A) \cup (\text{FIRST}(\beta_{i + 1}) - \{\epsilon\})$  
			$i \to i + 1$  
		if (i == k and $\epsilon \in \text{FIRST}(\beta_k)$)  
			$\text{FIRST}(A) \to \text{FIRST}(A) \cup \{\epsilon\}$  

## Example

### Expression Grammar

```
1. E  ->   T E'
2. E' -> + T E'
3.    |    e
4. T  ->   F T'
5. T' -> * F T'
6.    |    e
7. F  ->  (E)
8.    |    ID
```

$$\text{FIRST}(id) = \{ id \}$$

$$\text{FIRST}('(') = \{ ( \}$$

$$\text{FIRST}('+') = \{ + \}$$

$$\text{FIRST}(E) = \text{FIRST}(T) - \{ \varepsilon \}$$

$$\text{FIRST}(T) = \text{FIRST}(F) - \{ \varepsilon \}$$

$$\text{FIRST}(F) = \text{FIRST}('(') - \{ \varepsilon \} = \{ ( \}$$

$$\text{FIRST}(F) = \{ '(' \} + \text{FIRST}(id) - \{ \varepsilon \} = \{ (, id \}$$

$$\text{FIRST}(E') = \{ +, \varepsilon \}$$

$$\text{FIRST}(T') = \{ *, \varepsilon \}$$

Then  

$$\text{FIRST}(E) = \text{FIRST}(T) = \text{FIRST}(F) = \{ (, id \}$$

$$\text{FIRST}(E') = \{ +, \varepsilon \}$$

$$\text{FIRST}(T') = \{ *, \varepsilon \}$$

## `Follow Sets`[^2]

### Definition

$$\text{FOLLOW}(X) = \{b | S \to *\beta X b \omega\}$$

### Strategy

1. Add `$` to $\text{FOLLOW}(S)$ where $S$ is the start `non terminal`.
2. If $A \to \alpha B \beta$ exists then everything in $\text{FIRST}(\beta) - \{\epsilon\}$ is in $\text{FOLLOW}(B)$.
3. If $A \to \alpha B$ or $A \to \alpha B \beta$ exists where $\epsilon \in \text{FIRST}(\beta)$ then everything in $\text{FOLLOW}(A)$ is in $\text{FOLLOW}(B)$.

### Procedure

for each $A \in NT$ $\text{FOLLOW}(A) \to \emptyset$  
	$\text{FOLLOW}(S) \to \{\$\}$  
while (`FOLLOW sets`[^2] are still changing)  {  
	for each $A \to \beta_1 \beta_2 \ldots \beta_k \in P$ {  
		$\text{FOLLOW}(\beta_k) \to \text{FOLLOW}(\beta_k) \cup \text{FOLLOW}(A)$  
		$T \to \text{FOLLOW}(A)$  
		for $i \to k$ down to $2$  {  
			if ($\epsilon \in \text{FIRST}(\beta_i)$)  
				$\text{FOLLOW}(\beta_{i - 1}) \to \text{FOLLOW}(\beta_{i - 1}) \cup (\text{FIRST}(\beta_i) - \{\epsilon\}) \cup T$  
			else {  
				$\text{FOLLOW}(\beta_{i - 1}) \to \text{FOLLOW}(\beta_{i - 1}) \cup \text{FIRST}(\beta_i)$  
				$T \to \emptyset$  
			}  
		}  
	}  
}

### Apply to Expression Grammar

Put `$` in $\text{FOLLOW}(E)$.  
By rule (2) applied to production ? ( E ), ‘)’ is also in $\text{FOLLOW}(E)$.  
Thus, $\text{FOLLOW}(E) = \{ ), \$\}$.  
By rule (3) applied to production $E \to T E'$ , $ and ‘)’ are in $\text{FOLLOW}(E')$.  
Thus, $\text{FOLLOW}(E) = \text{FOLLOW}(E') = \{ ), \$ \}$.  
Similarly, $\text{FOLLOW}(T) = \text{FOLLOW}(T') = \{ +, ), \$ \}$ and $\text{FOLLOW}(F) = \{ +, \cdot , ), \$ \}$.

# References

[^1]: Read more about [[cs606_13|FIRST sets]].
[^2]: Read more about [[cs606_14|FOLLOW sets]].