---
tags:
  - university-notes
university-name: Virtual University of Pakistan
date: 2025-07-05
---

# 36. Space Curves

<span style="color: gray;">Dated: 05-07-2025</span>

$$\vec x(u) = a_x u^3 + b_x u^2 + c_xu + d_x$$

  Similarly, $\vec y(u)$ and $\vec z(u)$ will be  

$$\vec y(u) = a_y u^3 + b_y u^2 + c_yu + d_y$$

$$\vec z(u) = a_z u^3 + b_z u^2 + c_zu + d_z$$

Combining these into one equation, we have

$$\vec p(u) = au^3 + bu^2 + cu + d$$

Again, we will limit $u$ to $[0, 1]$ and let's take 4 points this time.

- Starting point ($u = \frac 0 3$)
- Intermediate point 1 ($u = \frac 1 3$)
- Intermediate point 2 ($u = \frac 2 3$)
- Ending point ($u = \frac 3 3$)

Substituting $u$ in $\vec x(u)$

$$
\begin{aligned}
	& x_1 = d_x \\
	& x_2 = \frac{1}{27}a_x + \frac{1}{9}b_x + \frac{1}{3}c_x + d_x \\
	& x_3 = \frac{8}{27}a_x + \frac{4}{9}b_x + \frac{2}{3}c_x + d_x \\
	& x_4 = a_x + b_x + c_x + d_x
\end{aligned}
$$

Finding the variables $a_x, b_x, c_x$ and $d_x$, we have

$$
\begin{aligned}
	& a_x = -\frac{9}{2}x_1 + \frac{27}{2}x_2 - \frac{27}{2}x_3 + \frac{9}{2}x_4 \\
	& b_x = 9x_1 - \frac{45}{2}x_2 + 18x_3 - \frac{9}{2}x_4 \\
	& c_x = -\frac{11}{2}x_1 + 9x_2 - \frac{9}{2}x_3 + x_4 \\
	& d_x = x_1
\end{aligned}
$$

Substituting back into $\vec x(u)$, we have

$$
x(u) = \left(-\frac{9}{2}x_1 + \frac{27}{2}x_2 - \frac{27}{2}x_3 + \frac{9}{2}x_4\right) u^3 + \left(9x_1 - \frac{45}{2}x_2 + 18x_3 - \frac{9}{2}x_4\right) u^2 \\
+ \left(-\frac{11}{2}x_1 + 9x_2 - \frac{9}{2}x_3 + x_4\right) u + x_1
$$

Refactoring it, we have

$$
x(u) = \left(-\frac{9}{2}u^3 + 9u^2 - \frac{11}{2}u + 1\right)x_1 + \left(\frac{27}{2}u^3 - \frac{45}{2}u^2 + 9u\right)x_2 \\
+ \left(-\frac{27}{2}u^3 + 18u^2 - 9u\right)x_3 + \left(\frac{9}{2}u^3 - \frac{9}{2}u^2 + u\right)x_4
$$

After finding the equivalent expressions for $\vec y (u)$ and $\vec z(u)$, we have

$$
\vec P(u) = \left(-\frac{9}{2}u^3 + 9u^2 - \frac{11}{2}u + 1\right)p_1 + \left(\frac{27}{2}u^3 - \frac{45}{2}u^2 + 9u\right)p_2 \\
+ \left(-\frac{27}{2}u^3 + 18u^2 - 9u\right)p_3 + \left(\frac{9}{2}u^3 - \frac{9}{2}u^2 + u\right)p_4
$$

Let

$$
\begin{array}{cc}
	G_1 = \left(-\frac{9}{2}u^3 + 9u^2 - \frac{11}{2}u + 1\right)
	& G_2 = \left(\frac{27}{2}u^3 - \frac{45}{2}u^2 + 9u\right) \\
	G_3 = \left(-\frac{27}{2}u^3 + 18u^2 - 9u\right)
	& G_4 = \left(\frac{9}{2}u^3 - \frac{9}{2}u^2 + u\right)
\end{array}
$$

such that

$$\vec P(u) = G_1p_1 + G_2p_2 + G_3 p_3 + G_4 p_4$$

$$\vec P(u) = GP$$

where

$$
G = 
\begin{bmatrix}
	G_1 & G_2 & G_3 & G_3
\end{bmatrix}
$$

$$
P = 
\begin{bmatrix}
	p_1 & p_2 & p_3 & p_3
\end{bmatrix}^T
$$

But $G$ can be further decomposed into

$$G = U N$$

Where

$$
U = \begin{bmatrix} u^3 & u^2 & u & 1 \end{bmatrix}^T
$$

$$
N = 
\begin{bmatrix}
	-\frac{9}{2} & \frac{27}{2} & -\frac{27}{2} & \frac{9}{2} \\
	9 & -\frac{45}{2} & 18 & -\frac{9}{2} \\
	-\frac{11}{2} & 9 & -\frac{9}{2} & 1 \\
	1 & 0 & 0 & 0
\end{bmatrix}
$$

$$
A = \begin{bmatrix}
	a \\
	b \\
	c \\
	d
\end{bmatrix} 
=
\begin{bmatrix}
	a_x & a_y & a_z \\
	b_x & b_y & b_z \\
	c_x & c_y & c_z \\
	d_x & d_y & d_z
\end{bmatrix}
$$

$$\vec p(u) = UA$$

$$\because \vec p(u) = \vec P(u)$$

$$UA = GP$$

$$\because G = UN$$

$$\implies UA = UNP$$

$$\implies A = NP$$
