---
tags:
  - university-notes
university-name: Virtual University of Pakistan
date: 2025-07-05
---

# 37. The `Tangent Vector`[^1]

<span style="color: gray;">Dated: 05-07-2025</span>

$$
\vec P^\prime(u)
=
\begin{bmatrix}
	\frac d {du} x(u) \hat i & 
	\frac d {du} y(u) \hat j & 
	\frac d {du} z(u) \hat k
\end{bmatrix}
$$

$$
\vec P^\prime(u)
=
\begin{bmatrix}
	x^\prime & y^\prime & z^\prime
\end{bmatrix}
$$

The `set`[^2] of `vectors`[^1] $p_0, p_1, p_0^\prime$ and $p_1^\prime$ are called boundary conditions.

This method itself is called the `cubic Hermite interpolation`, after `C. Hermite (1822-1901)` the French mathematician who made significant contributions to our understanding of cubic and quadratic polynomials.  

$$x(u) = a_x u^3 + b_x u^2 + c_x u + d_x$$

$$\frac d {du} x(u) = \frac d {du} \left(a_x u^3 + b_x u^2 + c_x u + d_x\right)$$

$$x^\prime = 3a_x u^2 + 2b_x u + c_x$$

$$x(0) = x_0 = d_x$$

$$x(1) = a_x + b_x + c_x + d_x$$

$$x^\prime(0) = x^\prime_0 = c_x$$

$$x^\prime(1) = x^\prime_1 = 3a_x + 2b_x + c_x$$

Solving for $a_x, b_x, c_x$ and $d_x$, we get

$$a_x = 2(x_0 - x_1) + x_0^\prime + x_1^\prime$$

$$b_x = 3(-x_0 + x_1) - 2x_0^\prime - x_1^\prime$$

$$c_x = x_0^\prime$$

$$d_x = x_0$$

Substituting in $\vec x(u)$, we get

$$
\vec x(u) = (2x_0 - 2x_1 + x_0^\prime + x_1^\prime) u^3 + (-3x_0 + 3x_1 - 2x_0^\prime - x_1^\prime x_0^\prime) u^2 + x_0^\prime + x_0
$$

$$
\vec x(u) = (2u^3 - 3u^2 + 1)x_0 + (-2u^3 + 3u^2)x_1 + (u^3 - 2u^2 + u)x_0^\prime + (u^3 - u^2)x_1^\prime
$$

Because $\vec y(u)$ and $\vec z(u)$ have equivalent forms

$$
\vec P(u) = (2u^3 - 3u^2 + 1)p_0 + (-2u^3 + 3u^2)p_1 + (u^3 - 2u^2 + u)p_0^\prime + (u^3 - u^2)p_1^\prime
$$

Let

$$
\begin{aligned}
	& F_1 = 2u^3 - 3u^2 + 1 \\
	& F_2 = -2u^3 + 3u^2 \\
	& F_3 = u^3 - 2u^2 + u \\
	& F_4 = u^3 - u^2
\end{aligned}
$$

$$
F =
\begin{bmatrix}
	F_1 & F_2 & F_3 & F_4
\end{bmatrix}
$$

$$
B = 
\begin{bmatrix}
	p_0 & p_1 & p_0^\prime & p_1^\prime
\end{bmatrix}^T
$$

$$
\vec P(u) = F_1 p_0 + F_2 p_1 + F_3 p_0^\prime + F_4 p_1^\prime
$$

$$\vec P(u) = FB$$

$F$ can be further decomposed into  

$$F = UM$$

where 

$$
U = \begin{bmatrix} u^3 & u^2 & u & 1 \end{bmatrix}
$$

$$
M = 
\begin{bmatrix}
	2 & -2 & 1 & 1 \\
	-3 & 3 & -2 & -1 \\
	0 & 0 & 1 & 0 \\
	1 & 0 & 0 & 0
\end{bmatrix}
$$

$$\vec P(u) = UMB$$

$$\vec p_0^\prime = \hat {p_0^\prime} \cdot |p_0^\prime|$$

$$\vec p_1^\prime = \hat {p_1^\prime} \cdot |p_1^\prime|$$

$$
\therefore \vec P(u) = (2u^3 - 3u^2 + 1)p_0 + (-2u^3 + 3u^2)p_1 + (u^3 - 2u^2 + u)\hat {p_0^\prime} \cdot |p_0^\prime| + (u^3 - u^2)\hat {p_1^\prime} \cdot |p_1^\prime|
$$

$$
\implies
B =
\begin{bmatrix}
	p_0 \\
	p_1 \\
	\hat {p_0^\prime} \cdot |p_0^\prime|\\
	\hat {p_1^\prime} \cdot |p_1^\prime|\\
\end{bmatrix}
$$

## References

[^1]: Read more about [[mth301_10|vectors]].
[^2]: Read more about [[M_Set|sets]].