---
tags:
  - university-notes
university-name: Virtual University of Pakistan
date: 2025-07-05
---

# 38. Bezier Curves

<span style="color: gray;">Dated: 05-07-2025</span>

In the early `1960s`, `Peter Bezier` began looking for a better way to define curves and surfaces one that would be useful to a design engineer.

## A Geometric Construction

![[cs602_e_38_1.svg]]  
/// caption  
Select 3 points $A, B$ and $C$.  
///

![[cs602_e_38_2.svg]]  
/// caption  
Select 2 points $D$ and $E$ such that $\frac {|\overline{AD}|}{|\overline{AB}|} = \frac {|\overline{BE}|}{|\overline{BC}|} = u_i$  
///

![[cs602_e_38_3.svg]]  
/// caption  
Select $F$ such that $\frac {|\overline{DF}|}{|\overline{FE}|} = u_i$, the curve is traced by $F$.  
///

Let $A = (x_A, y_A)$ and $B = (x_B, y_B)$ then `coordinates` of $D$ and $E$ are

$$
\begin{aligned}
	x_D = x_A + u_i(x_B - x_A) \\
	y_D = y_A + u_i(y_B - y_A)
\end{aligned}
$$

$$
\begin{aligned}
	x_E = x_B + u_i(x_C - x_B) \\
	y_E = y_B + u_i(y_C - y_B)
\end{aligned}
$$

Similarly, for $F$, we have

$$
\begin{aligned}
	x_F = x_D + u_i(x_E - x_D) \\
	y_F = y_D + u_i(y_E - y_D)
\end{aligned}
$$

Substituting coordinates for $D$ and $E$ in $F$ and after simplification, we have

$$
\begin{aligned}
	x_F = (1-u_i)^2 x_A + 2u_i(1-u_i) x_B + u_i^2 x_C \\
	y_F = (1-u_i)^2 y_A + 2u_i(1-u_i) y_B + u_i^2 y_C
\end{aligned}
$$

To generalize

$$
\begin{aligned}
	x(u) = x_F \\
	y(u) = y_F \\
\end{aligned}
$$

$$
\begin{array}{ccc}
	x_0 = x_A & x_1 = x_B & x_2 = x_C \\
	y_0 = y_A & y_1 = y_B & y_2 = y_C \\
\end{array}
$$

$$
\begin{aligned}
	x(u)=(1-u)^2 x_0 + 2u(1-u)x_1 + u^2 x_2 \\
	y(u)=(1-u)^2 y_0 + 2u(1-u)y_1 + u^2 y_2
\end{aligned}
$$

$$
p(u) = (1-u)^2 p_0 + 2u(1-u)p_1 + u^2 p_2
$$

Where $A = p_0, B = p_1, C = p_2$.

This is the `set`[^1] of second-degree equations for the coordinates of points on `Bezier curve` based on our construction.

> [!NOTE] The `degree` of a `Bezier curve` is equal to $n - 1$, where $n$ is the number of `control points`.

> [!TIP]- Cubic version  
> $p(u) = (1-u)^3 p_0 + 3u(1-u)^2 p_1 + 3u^2(1-u)p_2 + u^3 p_3$

$$p(u) = \sum_{i = 0}^n \binom{n}{i} u^i(1 - u)^{n - i} p_i \quad n = \text{Degree of Bezier curve}$$

## An Algebraic Definition

Bezier began with the idea that any point $p(u)$ on a curve segment should be given by an equation such as the following

$$
p(u) = \sum_{i=0}^n p_i f_i(u)
$$

![[cs602_i_38_1.png]]  
/// caption  
Source: [gamemath.com](https://gamemath.com/book/curves.html)  
///

The $f_i(u)$ has following important characteristics.

- The curve must start on the first control point, $p_0$, and end on the last, $p_n$. Mathematically, we say that the functions must `interpolate` these two points.
- The curve must be `tangent`[^2] to the `line`[^3] given by $p_1 - p_0$ at $p_0$ or $p_n - p_{n - 1}$ at $p_n$.
- The `functions`[^4] $f_i(u)$ must be symmetric with respect to $u$ and $(1 - u)$. This lets us reverse the sequence of control points without changing the shape of the `curve`.

![[cs602_i_38_2.png]]  
/// caption  
Effect of reversing the order of control points on the `curve`.  
///

We can rewrite the equation as

$$
p(u) = \sum_{i=0}^n p_i B_{i,n}(u)
$$

$$
B_{i,n}(u) = \binom{n}{i} u^i (1-u)^{n-i}
$$

where

$$
\binom{n}{i} = \frac{n!}{i!(n-i)!}
$$

Expanding this equation for `second degree Bezier curve`, we have

$$
p(u) = p_0 B_{0,2}(u) + p_1 B_{1,2}(u) + p_2 B_{2,2}(u)
$$

$$
\begin{aligned}
	B_{0,2}(u) & = (1-u)^2 \\
	B_{1,2}(u) & = 2u(1-u) \\
	B_{2,2}(u) & = u^2 \\
\end{aligned}
$$

similarly, for $n = 3$

$$
p(u) = p_0 B_{0,3}(u) + p_1 B_{1,3}(u) + p_2 B_{2,3}(u) + p_3 B_{3,3}(u)
$$

$$
\implies
p(u) = (1-u)^3 p_0 + 3u(1-u)^2 p_1 + 3u^2(1-u)p_2 + u^3 p_3
$$

$$
\implies
\begin{aligned}
	B_{0,3}(u) & = (1-u)^3 \\
	B_{1,3}(u) & = 3u(1-u)^2 \\
	B_{2,3}(u) & = 3u^2(1-u) \\
	B_{3,3}(u) & = u^3
\end{aligned}
$$

$$
\implies
p(u)
=
\begin{bmatrix}
	(1-u)^3 \\
	3u(1-u)^2 \\
	3u^2(1-u) \\
	u^3
\end{bmatrix}^T
\begin{bmatrix}
	p_0 \\
	p_1 \\
	p_2 \\
	p_3 \\
\end{bmatrix}
$$

$$
\begin{bmatrix}
	(1-3u+3u^2-u^3) \\
	(3u-6u^2+3u^3) \\
	(3u^2-3u^3) \\
	u^3
\end{bmatrix}^T
\begin{bmatrix}
	p_0 \\
	p_1 \\
	p_2 \\
	p_3
\end{bmatrix}
$$

$$
\begin{array}{cccc}
p(u) =
&
\begin{bmatrix}
	u^3 & u^2 & u & 1
\end{bmatrix}
&
\begin{bmatrix}
	-1 & 3 & -3 & 1 \\
	3 & -6 & 3 & 0 \\
	-3 & 3 & 0 & 0 \\
	1 & 0 & 0 & 0
\end{bmatrix}
&
\begin{bmatrix}
	p_0 \\ p_1 \\ p_2 \\ p_3
\end{bmatrix} \\
&
\Big \downarrow & \Big \downarrow & \Big \downarrow \\
& 
U & M & P
\end{array}
$$

$$p(u) = UMP$$

## References

[^1]: Read more about [[M_Set|sets]].
[^2]: Read more about [[mth301_10|vectors]].
[^3]: Read more about [[mth101_04|lines]].
[^4]: Read more about [[M_Function|functions]].