---
tags:
  - university-notes
university-name: Virtual University of Pakistan
date: 2025-07-04
---

# 35. Curves

<span style="color: gray;">Dated: 04-07-2025</span>

## Parametric Equations of a Curve

A `parametric curve` is one whose defining equations are given in terms of a single, common, independent variable called the `parametric variable`.  
A 3D `curve` will have $x, y$ and $z$ coordinates, each of which could be defined by a `function`[^1] of an independent variable $u$ such as  

$$x = x(u), \ y = y(u), \ z = z(u)$$

Let $p$ be a `vector`[^2] then

$$
\vec p (u) =
\begin{bmatrix}
	x(u) & y(u) & z(u)
\end{bmatrix}
$$

## Plane Curves

$$\vec x (u)= a_x u^2 + b_x u + c$$

$$\vec y (u)= a_y u^2 + b_y u + c$$

$$\vec z (u)= a_z u^2 + b_z u + c$$

We can combine these into

$$\vec p(u) = au^2 + bu + c$$

We will bound $u$ to $[0, 1]$ and each coefficient (i.e. $a, b$ and $c$) have their three components

$$
a =
\begin{bmatrix}
	a_x & a_y & a_z
\end{bmatrix}
$$

$$
b =
\begin{bmatrix}
	b_x & b_y & b_z
\end{bmatrix}
$$

$$
c =
\begin{bmatrix}
	c_x & c_y & c_z
\end{bmatrix}
$$

We can use 3 points to define a unique curve.

- Starting point ($u = 0$)
- Intermediate point ($u = 0.5$)
- Ending point ($u = 1$)

$$
p_0 = 
\begin{bmatrix}
	x_0 & y_0 & z_0
\end{bmatrix}
$$

$$
p_{0.5} = 
\begin{bmatrix}
	x_{0.5} & y_{0.5} & z_{0.5}
\end{bmatrix}
$$

$$
p_1 = 
\begin{bmatrix}
	x_{1} & y_{1} & z_{1}
\end{bmatrix}
$$

The subscripts represent the $u$ values.  
Now try solving the equations for $\vec x(u)$

$$x_0 = c_x$$

$$x_{0.5} = 0.25a_x + 0.5 b_x + c_x$$

$$x_1 = a_x + b_x + c_x$$

Solve for $a_x, b_x$ and $c_x$ and we have

$$a_x = 2x_0 - 4x_{0.5} + 2x_1$$

$$b_x = -3x_0 + 4x_{0.5} + x_1$$

$$c_x = x_0$$

Submitting these back into $\vec x(u)$, we get

$$
x(u) = (2x_0 - 4x_{0.5} + 2x_1) u^2 + (-3x_0 + 4x_{0.5} - x_1)u + x_0
$$

$$
= (2u^2 - 3u + 1) x_0 + (-4u^2 + 4u)x_{0.5} + (2u^2 - u) x_1
$$

Combining similar expressions for $\vec y(u)$ and $\vec z(u)$, we have

$$
\vec P(u) = (2u^2 - 3u + 1) p_0 + (-4u^2 + 4u)p_{0.5} + (2u^2 - u) p_1
$$

We can rewrite $\vec p(u)$ as follows

$$
\begin{bmatrix} u^2 & u & 1 \end{bmatrix} \begin{bmatrix} a \\ b \\ c \end{bmatrix} = au^2 + bu + c
$$

$$
U = \begin{bmatrix} u^2 & u & 1 \end{bmatrix}
$$

$$
A = \begin{bmatrix} a & b & c \end{bmatrix}^T
$$

$$\vec p(u) = UA$$

$$
	A = \begin{bmatrix}
	a \\
	b \\
	c
	\end{bmatrix} = \begin{bmatrix}
	a_x & a_y & a_z \\
	b_x & b_y & b_z \\
	c_x & c_y & c_z
	\end{bmatrix}
$$

Now we will rewrite $\vec P(u)$ in similar way

$$
\vec P(u) = \begin{bmatrix} (2u^2 - 3u + 1) & (-4u^2 + 4u) & (2u^2 - u) \end{bmatrix} \begin{bmatrix} p_0 \\ p_{0.5} \\ p_1 \end{bmatrix}
$$

$$
F = \begin{bmatrix} (2u^2 - 3u + 1) & (-4u^2 + 4u) & (2u^2 - u) \end{bmatrix}
$$

$$
	P = \begin{bmatrix}
	p_0 \\
	p_{0.5} \\
	p_1
	\end{bmatrix} = \begin{bmatrix}
	x_0 & y_0 & z_0 \\
	x_{0.5} & y_{0.5} & z_{0.5} \\
	x_1 & y_1 & z_1
	\end{bmatrix}
$$

$$\vec P(u) = FP$$

Because the 2 are equations for same curve

$$\vec p(u) = \vec P(u)$$

$$UA = FP$$

We can decompose $F$ into

$$
F = \begin{bmatrix} u^2 & u & 1 \end{bmatrix} \begin{bmatrix}
	2 & -4 & 2 \\
	-3 & 4 & -1 \\
	1 & 0 & 0
\end{bmatrix}
$$

Let 

$$
M = \begin{bmatrix}
	2 & -4 & 2 \\
	-3 & 4 & -1 \\
	1 & 0 & 0
\end{bmatrix}
$$

So  

$$F = UM$$

Therefore, we have  

$$UMP = UA$$

$$\implies MP = A$$

$$\implies M^{-1}MP = M^{-1}A$$

The `matrix`[^3] $M$ is called a `basis transformation matrix`, and $F$ is called a `blending function matrix`.

## References

[^1]: Read more about [[M_Function|functions]].
[^2]: Read more about [[mth301_10|vectors]].
[^3]: Read more about [[mth501_02|matrices]].