---
tags:
  - university-notes
university-name: Virtual University of Pakistan
date: 2025-06-12
---

# 29. The Characteristic Equation

<span style="color: gray;">Dated: 12-06-2025</span>

$$\det(A - \lambda I) = \vec 0$$

Here $\lambda$ is the `eigenvalue`[^1] and $I$ is the `identity matrix`.[^2] This equation is also called `characteristic polynomial`.

## Example

Find `eigen values`[^1] of

$$
A 
=
\begin{bmatrix}
	2 & 3\\
	3 & -6
\end{bmatrix}
$$

$$(A - \lambda I) \vec x = \vec 0$$

$$
A - \lambda I 
=
\begin{bmatrix}
	2 & 3 \\
	3 & -6
\end{bmatrix}
-
\begin{bmatrix}
	\lambda & 0 \\
	0 & \lambda
\end{bmatrix}
=
\begin{bmatrix}
	2-\lambda & 3 \\
	3 & -6-\lambda
\end{bmatrix}
$$

By definition  

$$
\det(A - \lambda I) = 
\det 
\left(
\begin{bmatrix}
	2-\lambda & 3 \\
	3 & -6-\lambda
\end{bmatrix}
\right)
= 0
$$

$$
\det 
\left(
\begin{bmatrix}
	a & b \\
	c & d
\end{bmatrix}
\right)
= ad-bc
$$

$$\det(A-\lambda I) = (2-\lambda)(-6-\lambda)-(3)(3)$$

$$= -12+6\lambda-2\lambda+\lambda^2-9$$

$$= \lambda^2+4\lambda-21$$

$$\lambda^2+4\lambda-21=0$$

$$(\lambda-3)(\lambda+7)=0$$

Hence, the `eigen values`[^1] are $3$ and $-7$.

## Similarity

$A_{n \times n}$ and $B_{n \times n}$ are similar if there exists and `invertible matrix`[^3] $P$ such that

$$P^{-1}AP = B$$

$$A = PBP^{-1}$$

## Similarity Transformation

The act of changing $A$ into $P^{-1} A P$ is called a `similarity transformation`.

## Theorem

If $A_{n \times n}$ and $B_{n \times n}$ are similar then they have same `characteristic polynomial` and hence the same `eigenvalues`.[^1]

> [!Warning] `Row operations`[^4] on a matrix usually change its `eigenvalues`.[^1]

## Application to Dynamic Systems

Let

$$
A =
\begin{bmatrix}
	.95 & .03 \\
	.05 & .97
\end{bmatrix}
$$

Analyze the behavior of long term dynamical system defined by

$$\vec x_{k + 1} = A \vec x_k \quad k = 0, 1, 2, \ldots$$

with  

$$
x_0
=
\begin{bmatrix}
	0.6 \\
	0.4
\end{bmatrix}
$$

First step is to find `eigen values`[^1] of $A$ and a `basis` for each `eigenspace`.[^1]

$$\det(A - \lambda I) = 0$$

$$
0 =
\det
\left(
\begin{bmatrix}
	0.95 - \lambda & 0.03 \\
	0.05 & 0.97 - \lambda
\end{bmatrix}
\right)
=
(0.95-\lambda)(0.97-\lambda) - (0.03)(0.05)
$$

$$= \lambda^2 - 1.92\lambda + 0.92$$

Applying quadratic formula  

$$\lambda = \frac{1.92 \pm \sqrt{(1.92)^2 - 4(0.92)}}{2} = \frac{1.92 \pm \sqrt{0.0064}}{2} = \frac{1.92 \pm 0.08}{2} = 1 \text{ or } 0.92$$

$$Ax = \lambda x$$

$$(Ax - \lambda x) = 0$$

$$(A-\lambda I)x = 0$$

### For $\lambda = 1$

$$
\begin{bmatrix}
	0.95 & 0.03 \\
	0.05 & 0.97
\end{bmatrix}
-
\begin{bmatrix}
	1 & 0 \\
	0 & 1
\end{bmatrix}
\begin{bmatrix}
	x_1 \\
	x_2
\end{bmatrix} = 0
$$

$$
\begin{bmatrix}
	-0.05 & 0.03 \\
	0.05 & -0.03 \\
\end{bmatrix}
\begin{bmatrix}
	x_1 \\
	x_2 \\
\end{bmatrix}
= 0
$$

$$-0.05x_1 + 0.03 = 0$$

$$0.05x_1 - 0.03x_2 = 0 \implies x_1 = \frac{0.03}{0.05}x_2 \implies x_1 = \frac{3}{5}x_2$$

In parametric form, it becomes

$$x_1 = \frac{3}{5}t \text{ and } x_2 = t$$

### For $\lambda = 0.92$

$$
\begin{bmatrix}
	0.95 & 0.03 \\
	0.05 & 0.97
\end{bmatrix}
-
\begin{bmatrix}
	0.92 & 0 \\
	0 & 0.92
\end{bmatrix}
\begin{bmatrix}
	x_1 \\
	x_2
\end{bmatrix}
= 0
$$

$$
\begin{bmatrix}
	0.03 & 0.03 \\
	0.05 & 0.05 \\
\end{bmatrix}
\begin{bmatrix}
	x_1 \\
	x_2 \\
\end{bmatrix}
= 0
$$

$$0.03x_1 + 0.03x_2 = 0$$

$$0.05x_1 + 0.05x_2 = 0 \implies x_1 = -x_2$$

$$x_1 = t \text{ and } x_2 = -t$$

Thus, the `eigen vectors`[^1] corresponding to $\lambda = 1$ and $\lambda = .92$ are

$$
v_1
=
\begin{bmatrix}
	3 \\
	5
\end{bmatrix}
$$

$$
v_2
=
\begin{bmatrix}
	1 \\
	-1
\end{bmatrix}
$$

Next step is to write $x_0$ in terms of $v_1$ and $v_2$.  
$\{v_1, v_2\}$ is `basis` for $\mathbb R^2$.  
So there exists weights $c_1$ and $c_2$ such that

$$
x_0 = c_1 \vec{v}_1 + c_2 \vec{v}_2 =
\begin{bmatrix}
	\vec{v}_1 & \vec{v}_2
\end{bmatrix}
\begin{bmatrix}
	c_1 \\
	c_2
\end{bmatrix}
$$

$$
\begin{bmatrix}
	 c_1 \\
	 c_2 \\
\end{bmatrix}
=
\begin{bmatrix}
	\vec{v}_1 & \vec{v}_2
\end{bmatrix}^{-1} x_0
=
\begin{bmatrix}
	3 & 1 \\
	5 & -1 \\
\end{bmatrix}^{-1}
\begin{bmatrix}
	0.60 \\
	0.40 \\
\end{bmatrix}
$$

$$
\begin{bmatrix}
	3 & 1 \\
	5 & -1 \\
\end{bmatrix}^{-1}
=
\frac{1}{
	\begin{vmatrix} 
		3 & 1 \\
		5 & -1 \\
	\end{vmatrix}
}
\text{Adj}
\begin{bmatrix}
	3 & 1 \\
	5 & -1 \\
\end{bmatrix}
=
\frac{1}{-8}
\begin{bmatrix}
	-1 & -1 \\
	-5 & 3 \\
\end{bmatrix}
$$

$$
\begin{bmatrix}
	c_1 \\
	c_2 \\
\end{bmatrix}
=
\frac{1}{-8}
\begin{bmatrix}
	-1 & -1 \\
	-5 & 3 \\
\end{bmatrix}
\begin{bmatrix}
	0.60 \\
	0.40 \\
\end{bmatrix}
=
\begin{bmatrix}
	0.125 \\
	0.225 \\
\end{bmatrix}
$$

Since $v_1$ and $v_2$ are `eigen vectors`[^1] of $A$ then  

$$A v_1 = (1)v_1$$

$$A v_2 = (0.92)v_2$$

$$\vec x_1 = A \vec x_0$$

$$= c_1 A v_1 + c_2 A v_2$$

$$= c_1 v_1 + c_2 (0.92) v_2$$

$$x_2 = A x_1 = c_1 A v_1 + c_2 (0.92) A v_2 = c_1 v_1 + c_2 (0.92)^2 v_2$$

$$\vec{x}_k = c_1 \vec{v}_1 + c_2 (0.92)^k \vec{v}_2 \quad k \ge 0$$

$$
\vec{x}_k
=
0.125
\begin{bmatrix}
	3 \\
	5
\end{bmatrix}
+
0.225 (0.92)^k
\begin{bmatrix}
	1 \\
	-1
\end{bmatrix}
\quad k \ge 0
$$

As  

$$
k \to \infty \implies (0.92)^k \to 0 \implies
\vec x_k =
\begin{bmatrix}
	.375 \\
	.625
\end{bmatrix}
= 
.125 \vec v_1
$$

## References

Read more about [[M_Notations|notations and symbols]].

[^1]: Read more about [[mth501_28|eigen values and vectors]].
[^2]: Read more about [[mth501_02|matrices]].
[^3]: Read more about [[mth501_12|invertible matrices]].
[^4]: Read more about [[mth501_03|row operations]].