---
tags:
  - university-notes
university-name: Virtual University of Pakistan
date: 2024-11-22
---

# 14. Solutions to Higher order Linear Equations

<span style="color: gray;">Dated: 22-11-2024</span>

## Preliminary Theory

In order to solve an $nth$ order non-homogenous linear differential equation  

$$a_{n}(x)\frac{d^{n}y}{dx^{n}}+a_{n-1}(x)\frac{d^{n-1}y}{dx^{n-1}}+\cdot\cdot\cdot+a_{1}(x)\frac{dy}{dx}+a_{0}(x)y=g(x)$$

We first solve for  

$$a_{n}(x)\frac{d^{n}y}{dx^{n}}+a_{n-1}(x)\frac{d^{n-1}y}{dx^{n-1}}+\cdot\cdot\cdot+a_{1}(x)\frac{dy}{dx}+a_{0}(x)y=0$$

## Super Position

Suppose $y_1, y_2, \ldots, y_n$ are solutions on the interval $I$ for

$$a_{n}(x)\frac{d^{n}y}{dx^{n}}+a_{n-1}(x)\frac{d^{n-1}y}{dx^{n-1}}+\cdot\cdot\cdot+a_{1}(x)\frac{dy}{dx}+a_{0}(x)y=0$$

then the following is also a solution.  

$$y=c_{1}y_{1}(x)+c_{2}y_{2}(x)+\cdot\cdot\cdot+c_{n}y_{n}(x)$$

where $c_1, c_2, c_n$ are arbitrary `constants`.

> [!NOTE] Notes
> - If $y_1(x)$ is a solution to `homogeneous linear differential equation`[^1] then $y = cy_1(x)$ is also a solution.
> - `Homogeneous linear differential equations`[^1] always possess trivial solution $y = 0$.
> - The [super position principle](#super-position) does not holds for non `linear differential equations`.[^2]

## Example

The `functions`[^3]  

$$y_1 = e^x$$

$$y_2 = c^{2x}$$

$$y_3 = e^{3x}$$

satisfy the `homogeneous differential equation`[^1]  

$$\frac{d^{3}y}{dx^{3}}-6\frac{d^{2}y}{dx^{2}}+11\frac{dy}{dx}-6y=0$$

on $(- \infty, \infty)$.  
This $y_1, y_2, y_3$ are all solutions.  
Now suppose  

$$y=c_{1}e^{x}+c_{2}e^{2x}+c_{3}e^{3x}$$

Then  

$$\frac{dy}{dx}=c_{1}e^{x}+2c_{2}e^{2x}+3c_{3}e^{3x}$$

$$\frac{d^{2}y}{dx^{2}}=c_{1}e^{x}+4c_{2}e^{2x}+9c_{3}e^{3x}$$

$$\frac{d^{3}y}{dx^{3}}=c_{1}e^{x}+8c_{2}e^{2x}+27c_{3}e^{3x}$$

Therefore

$$\frac{d^{3}y}{dx^{3}}-6\frac{d^{2}y}{dx^{2}}+11\frac{dy}{dx}-6y=c_{1}(e^{x}-6e^{x}+11e^{x}-6e^{x})+c_{2}(8e^{2x}-24e^{2x}+22e^{2x}-6e^{2x}) + c_3(27e^{3x} - 54e^{3x} + 33e^{3x} - 6e^{3x})$$

$$=c_{1}(12-12)e^{x}+c_{2}(30-30)e^{2x}+c_{3}(60-60)e^{3x}$$

 $$= 0$$

Therefore,

$$y=c_{1}e^{x}+c_{2}e^{2x}+c_{3}e^{3x}$$

is also a solution.

## The Wronskian

Suppose that $y_1, y_2$ are solutions on `interval`[^4] $I$ of the following.  

$$a_{2}\frac{d^{2}y}{dx^{2}}+a_{1}\frac{dy}{dx}+a_{0}y=0$$

Then either  

$$W(y_1, y_2) = 0, \forall x \in I$$

or

$$W(y_1, y_2) \ne 0, \forall x \in I$$

To verify this, we write  

$$\frac{d^{2}y}{dx^{2}}+P\frac{dy}{dx}+Qy=0$$

$$W(y_{1},y_{2})=\begin{vmatrix}y_{1}&y_{2}\\ y_{1}^{\prime}&y_{2}^{\prime}\end{vmatrix}=y_{1}y_{2}^{\prime}-y_{1}^{\prime}y_{2}$$

$$\implies \frac{dW}{dx} = y_1y_2^{\prime\prime} - y_1^{\prime\prime}y_2$$

We the re-write the equation in the following form  

$$y_{1}^{\prime\prime}+Py_{1}^{\prime}+Qy_{1}=0$$

$$y_{2}^{\prime\prime}+Py_{2}^{\prime}+Qy_{2}=0$$

Multiplying first equation by $y_2$ and second equation by $y_1$, we have  

$$y_{1}^{\prime\prime}y_{2}+Py_{1}^{\prime}y_{2}+Qy_{1}y_{2}=0$$

$$y_{1}y_{2}^{\prime\prime}+Py_{1}y_{2}^{\prime}+Qy_{1}y_{2}=0$$

Subtracting both, we have  

$$(y_{1}y_{2}^{\prime\prime}-y_{2}y_{1}^{\prime\prime})+P(y_{1}y_{2}^{\prime}-y_{1}^{\prime}y_{2})=0$$

Which can be re-written as  

$$\frac {dW}{dx} + PW = 0$$

And its solution is  

$$W=ce^{-\int Pdx}$$

Therefore

- If $c \ne 0$ then $W(y_1, _2) \ne 0, \quad \forall x \in I$.
- If $c = 0$ then $W(y_1, y_2) = 0, \quad \forall x \in I$.

### In General

If $y_1, y_2, \ldots, y_n$ are solutions on `interval`[^4] $I$ for 

$$a_{n}(x)\frac{d^{n}y}{dx^{n}}+a_{n-1}(x)\frac{d^{n-1}y}{dx^{n-1}}+\cdot\cdot\cdot+a_{1}(x)\frac{dy}{dx}+a_{0}(x)y=0$$

Then  

$$W(y_{1},y_{2},…,y_{n})=0, \forall x\in I$$

or  

$$W(y_{1},y_{2},…,y_{n})\neq 0, \forall x\in I$$

## Fundamental Set of Solutions

A `set`[^5] $\{y_1, y_2, \ldots, y_n\}$ of $n$ `linearly independent solutions`[^6] on `interval`[^4] $I$ for

$$a_{n}(x)\frac{d^{n}y}{dx^{n}}+a_{n-1}(x)\frac{d^{n-1}y}{dx^{n-1}}+\cdot\cdot\cdot+a_{1}(x)\frac{dy}{dx}+a_{0}(x)y=0$$

is called `fundamental set of solutions` on the `interval`[^4] $I$.

### Existence of Fundamental Set of Solutions

There always exists the `fundamental set of solutions` for equations of the form

$$a_{n}(x)\frac{d^{n}y}{dx^{n}}+a_{n-1}(x)\frac{d^{n-1}y}{dx^{n-1}}+\cdot\cdot\cdot+a_{1}(x)\frac{dy}{dx}+a_{0}(x)y=0$$

on `interval`[^4] $I$.

## General Solution for Homogeneous Equations

Suppose that  

$$\{y_1, y_2, \ldots, y_n\}$$

is a [fundamental set of solutions](#fundamental-set-of-solutions) on the `interval`[^4] $I$ for the equations  

$$a_{n}(x)\frac{d^{n}y}{dx^{n}}+a_{n-1}(x)\frac{d^{n-1}y}{dx^{n-1}}+\cdot\cdot\cdot+a_{1}(x)\frac{dy}{dx}+a_{0}(x)y=0$$

Then the general solution on the `interval`[^4] $I$ is defined to be  

$$y=c_{1}y_{1}(x)+c_{2}y_{2}(x)+\ldots+c_{n}y_{n}(x)$$

Where $c_1, c_2, \ldots, c_n$ are arbitrary constants.

## Example

Consider the equation  

$$\frac{d^{3}y}{dx^{3}}-6\frac{d^{2}y}{dx^{2}}+11\frac{dy}{dx}-6y=0$$

and suppose that  

$$y_1 = e^x$$

$$y_2 = e^{2x}$$

$$y_3 = e^{3x}$$

Then  

$$\frac{dy_{1}}{dx}=e^{x}=\frac{d^{2}y_{1}}{dx^{2}}=\frac{d^{3}y_{1}}{dx^{3}}$$

Therefore  

$$\frac{d^{3}y_{1}}{dx^{3}}-6\frac{d^{2}y_{1}}{dx^{2}}+11\frac{dy_{1}}{dx}-6y_{1}=12e^{x}-12e^{x}=0$$

Now for $x \in \mathbb R$.  

$$W(e^{x},e^{2x},e^{3x})=\begin{vmatrix}e^{x}&e^{2x}&e^{3x}\\ e^{x}&2e^{2x}&3e^{3x}\\ e^{x}&4e^{2x}&9e^{3x}\end{vmatrix}=2e^{6x}\neq0\forall x\in I$$

Therefore, $y_1, y_2$ and $y_n$ form a fundamental solution of the differential equation on $(- \infty, \infty)$.  

$$y = c_1e^{x} + c_2e^{2x} + c_3e^{3x}$$

## Non Homogeneous Equations

A `function`[^3] $y_p$ that satisfied the non-homogeneous differential equation.  

$$a_{n}(x)\frac{d^{n}y}{dx^{n}}+a_{n-1}(x)\frac{d^{n-1}y}{dx^{n-1}}+\cdot\cdot\cdot+a_{1}(x)\frac{dy}{dx}+a_{0}(x)y=g(x)$$

and is free of parameters is called the `particular solution of differential equation`.

### Example

Suppose that  

$$y_p = 3$$

Then  

$$y_p^{\prime\prime} = 0$$

So that  

$$y_p^{\prime\prime} + 9 y_p = 0 + 9(3)$$

$$= 27$$

Therefore  

$$y_p = 3$$

is the particular solution of the differential equation  

$$y_p^{\prime\prime} + 9y_p = 27$$

## Complementary Function

The general solution  

$$y=c_{1}y_{1}+c_{2}y_{2}+\ldots+c_{n}y_{n}$$

of the `homogeneous linear differential equation`

$$a_{n}(x)\frac{d^{n}y}{dx^{n}}+a_{n-1}(x)\frac{d^{n-1}y}{dx^{n-1}}+\ldots+a_{1}(x)\frac{dy}{dx}+a_{0}(x)y=0$$

is known as the `complmentary function` for the non-homogeneous linear differential equation.

$$a_{n}(x)\frac{d^{n}y}{dx^{n}}+a_{n-1}(x)\frac{d^{n-1}y}{dx^{n-1}}+\ldots+a_{1}(x)\frac{dy}{dx}+a_{0}(x)y=g(x)$$

## General Solution of Non-homogeneous Equations

$$\text{general solution} = \text{complementary solution} + \text{any particular solution}$$

### Example

Suppose that  

$$y_p = - \frac {11}{12} - \frac 1 2 x$$

Then  

$$y_p^\prime = - \frac 1 2, y_p^{\prime\prime} = y_p^{\prime\prime\prime} = 0$$

$$\therefore \frac{d^{3}y_{p}}{dx^{3}}-6\frac{d^{2}y_{p}}{dx^{2}}+11\frac{dy_{p}}{dx}-6y_{p}=0-0-\frac{11}{2}+\frac{11}{2}+3x=3x$$

Therefore, $y_p$ is the solution of non-homogeneous linear equation above.  
Now consider  

$$y_{c}=c_{1}e^{x}+c_{2}e^{2x}+c_{3}e^{3x}$$

Therefore  

$$\frac{dy_{c}}{dx}=c_{1}e^{x}+2c_{2}e^{2x}+3c_{3}e^{3x}$$

$$\frac{d^{2}y_{c}}{dx^{2}}=c_{1}e^{x}+4c_{2}e^{2x}+9c_{3}e^{3x}$$

$$\frac{d^{3}y_{c}}{dx^{3}}=c_{1}e^{x}+8c_{2}e^{2x}+27c_{3}e^{3x}$$

$$\frac{d^{3}y_{c}}{dx^{3}}-6\frac{d^{2}y_{c}}{dx^{2}}+11\frac{dy_{c}}{dx}-6y_{c} =c_{1}e^{x}+8c_{2}e^{2x}+27c_{3}e^{3x}-6(c_{1}e^{x}+4c_{2}e^{2x}+9c_{3}e^{3x}) +11(c_{1}e^{x}+2c_{2}e^{2x}+3c_{3}e^{3x})-6(c_{1}e^{x}+c_{2}e^{2x}+c_{3}e^{3x})$$

$$=12c_{1}e^{x}-12c_{1}e^{x}+30c_{2}e^{2x}-30c_{2}e^{2x}+60c_{3}e^{3x}-60c_{3}e^{3x}$$

$$=0$$

Thus, $y_c$ is the general solution of associated homogeneous differential equation.  

$$\frac{d^{3}y}{dx^{3}}-6\frac{d^{2}y}{dx^{2}}+11\frac{dy}{dx}-6y=0$$

Hence the general solution for non-homogeneous equation is  

$$y=y_{c}+y_{p}=c_{1}e^{x}+c_{2}e^{2x}+c_{3}e^{3x}-\frac{11}{12}-\frac{1}{2}x$$

## Super Position Principle for Non-homogeneous Equations

Suppose that  

$$y_{p_1}, y_{p_2}, \ldots, y_{p_k}$$

denotes the particular solutions of the $k$ differential equation.  

$$a_{n}(x)y^{(n)}+a_{n-1}(x)y^{(n-1)}+\cdot\cdot\cdot+a_{1}(x)y^{\prime}+a_{0}(x)y=g_{i}(x)$$

where $i = 1, 2, \ldots, k$ on an `interval`[^4] $I$.  
Then  

$$y_p = y_{p_1}(x) + y_{p_2}(x) + \cdots + y_{p_k}(x)$$

is a particular solution for  

$$a_{n}(x)y^{(n)}+a_{n-1}(x)y^{(n-1)}+\cdot\cdot\cdot+a_{1}(x)y^{\prime}+a_{0}(x)y=g_{1}(x)+g_{2}(x)+\cdot\cdot\cdot+g_{k}(x)$$

## Example

Consider the differential equation  

$$y^{\prime\prime}-3y^{\prime}+4y=-16x^{2}+24x-8+2e^{2x}+2xe^{x}-e^{x}$$

Suppose that  

$$y_{p_1} = - 4x^2$$

$$y_{p_2} = e^{2x}$$

$$y_{p_3} = xe^x$$

Then  

$$y_{p_1}^{\prime\prime}-3y_{p_1}^{\prime}+4y_{p_1}=-8+24x-16x^{2}$$

Therefore  

$$y_{p_1}=-4x^{2}$$

is a particular solution of the non homogeneous differential equation  

$$y^{\prime\prime}-3y^{\prime}+4y=-16x^{2}+24x-8$$

$$y_{p_2} = e^{2x}$$

$$y_{p_3} = xe^x$$

are particular solutions for  

$$y^{\prime\prime}-3y^{\prime}+4y=2e^{2x}$$

and  

$$y^{\prime\prime}-3y^{\prime}+4y=2xe^{x}-e^{x}$$

respectively.  
Hence,  

$$y=y_{p_1}+y_{p_2}+y_{p_3}=-4x^{2}+e^{2x}+xe^{x}$$

is the solution of the differential equation  

$$y^{\prime\prime}-3y^{\prime}+4y=-16x^{2}+24x-8+2e^{2x}+2xe^{x}-e^{x}$$

## References

Read more about [[M_Notations|notations and symbols]].

[^1]: Read more about [[mth401_04|homogeneous differential equations]].
[^2]: Read more about [[mth401_07|linear differential equations]].
[^3]: Read more about [[M_Function|functions]].
[^4]: Read more about [[mth101_01|intervals]].
[^5]: Read more about [[M_Set|sets]].
[^6]: Read more about [[mth401_13|linear dependence]].