---
tags:
  - university-notes
university-name: Virtual University of Pakistan
date: 2024-11-28
---

# 16. Homogeneous Linear Equations with Constant Coefficients

<span style="color: gray;">Dated: 28-11-2024</span>

We know that  

$$\frac{dy}{dx}+my=0$$

where $m$ being a constant, has the following solution on $(-\infty, \infty)$  

$$y = c_1e^{-mx}$$

## Recall

The equation  

$$a_{n}(x)\frac{d^{n}y}{dx^{n}}+a_{n-1}(x)\frac{d^{n-1}y}{dx^{n-1}}+â€¦+a_{1}(x)\frac{dy}{dx}+a_{0}(x)y=g(x)$$

for $n = 2$ becomes  

$$a_{2}\frac{d^{2}y}{dx^{2}}+a_{1}\frac{dy}{dx}+a_{0}y=0$$

Which can be re-written as  

$$a\frac{d^{2}y}{dx^{2}}+b\frac{dy}{dx}+cy=0$$

Now we try out a solution of exponential form  

$$y = e^{mx}$$

Then  

$$y^\prime = me^{mx}$$

$$y^{\prime\prime} = m^2e^{mx}$$

Substituting into original equation, we have  

$$e^{mx}(am^{2}+bm+c)=0$$

$$\because e^{mx}\neq 0, \forall x\in (-\infty,\infty)$$

$$\therefore am^{2}+bm+c=0$$

This algebraic equation is known as `auxiliary equation`.

### Case 1: Distinct Real Roots

If the `auxiliary equation` has distinct roots, $m_1$ and $m_2$ then the solutions are  

$$y_1 = e^{m_1x}$$

$$y_2 = e^{m_2x}$$

These solutions are `linearly independent`[^1]

$$W(y_1, y_2) = 
\begin{vmatrix}
	y_1 & y_2\\
	y_1^\prime & y_2^\prime
\end{vmatrix}
$$

$$= (m_2 - m_1) e^{(m_1 + m_2)x}$$

Since $m_1 \ne m_2$ and $e^{(m_1 + m_2)} \ne 0$  
Therefore,  

$$W(y_1, y_2) \ne 0, \forall x \in (- \infty, \infty)$$

$$y = c_1e^{m_1x} + c_2e^{m_2x}$$

### Case 2: Repeated Roots

if we have `real` roots such that $m_1 = m_2$ then we have only one solution  

$$y = c_1 e^{mx}$$

We can re-write the equation to the following form  

$$y''+\frac{b}{a}y'+\frac{c}{a}y=0$$

$$y''+Py'+Qy=0$$

$$P=\frac{b}{a}$$

Therefore, the second solution is  

$$y_2=y_1\int\frac{e^{-\int Pdx}}{(y_1)^2}dx=e^{mx}\int\frac{e^{-\frac{b}{a}x}}{e^{2mx}}dx$$

$$\because \text{Disc} = b^2 - 4ac = 0$$

$$m=\frac{-b\pm\sqrt{b^{2}-4ac}}{2a}$$

$$2m=-\frac{b}{a}$$

Therefore  

$$y_2=e^{mx}\int\frac{e^{2mx}}{e^{2mx}}dx=xe^{mx}$$

Hence the `general solution`[^2] is  

$$y=c_1e^{mx}+c_2xe^{mx}=(c_1+c_2x)e^{mx}$$

### Case 3: Complex Roots

If the `auxiliary equation` has the complex roots $\alpha \pm \iota \beta$ then  

$$m_1 = \alpha + \iota \beta$$

$$m_2 = \alpha - \iota \beta$$

Where $\alpha, \beta > 0$ and are `real`.  

$$y=c_{1}e^{(\alpha+i\beta)x}+c_{2}e^{(\alpha-i\beta)x}$$

Choosing the following pairs for $(c_1, c_2)$  

$$(1, 1)$$

$$(1, -1)$$

Thus we have  

$$y_{1}=e^{(\alpha+i\beta)x}+e^{(\alpha-i\beta)x}$$

$$y_{2}=e^{(\alpha+i\beta)x}-e^{(\alpha-i\beta)x}$$

By `Euler's Formula`  

$$e^{\iota \theta} = \cos (\theta) + \iota \sin(\theta), \theta \in \mathbb R$$

$$y_1=e^{\alpha x}(e^{i\beta x}+e^{-i\beta x})=2e^{\alpha x}\cos \beta x$$

$$y_2=e^{\alpha x}(e^{i\beta x}-e^{-i\beta x})=2ie^{\alpha x}\sin \beta x$$

We can drop the constants to write  

$$y_1 = e^{\alpha x} \cos (\beta x)$$

$$y_2 = e^{\alpha x} \sin (\beta x)$$

## The Wronskian

$$W(e^{\alpha x}\cos \beta x, e^{\alpha x}\sin \beta x)=\beta e^{2\alpha x}\neq 0 \quad \forall x$$

Therefore the following form a `fundamental solution`[^2] of the differential equation $(- \infty, \infty)$.

$$e^{\alpha x}\cos \beta x, e^{\alpha x}\sin \beta x$$

Therefore, the `general solution`[^2] is

$$y=c_1e^{\alpha x}\cos \beta x+c_2e^{\alpha x}\sin \beta x$$

$$y=e^{\alpha x}(c_1\cos \beta x+c_2\sin \beta x)$$

### Example

$$y^{\prime\prime} - 10y^{\prime}+25y=0$$

#### Solution

We put  

$$y=e^{mx}$$

$$y^{\prime}=me^{mx}, y^{\prime\prime}=m^2e^{mx}$$

Substituting in the given differential equation, we have  

$$(m^2 - 10m + 25)e^{mx} = 0$$

$$\because e^{mx} \ne 0, \forall x$$

$$m^2-10m+25=0$$

$$(m-5)^2=0\Rightarrow m=5,5$$

Hence,  

$$y=c_1e^{5x}+c_2xe^{5x}$$

$$y=(c_1+c_2x)e^{5x}$$

## Higher order Equations

If we consider the following $nth$ order `homogeneous`[^3] `linear differential equation`.[^4]

$$a_{n}\frac{d^{n}y}{dx^{n}}+a_{n-1}\frac{d^{n-1}y}{dx^{n-1}}+\ldots+a_{1}\frac{dy}{dx}+a_{0}y=0$$

then the `auxiliary equation` is  

$$a_{n}m^{n}+a_{n-1}m^{n-1}+\ldots+a_{1}m+a_{0}=0$$

### Case 1: Real Distinct Roots

$$y=c_{1}e^{m_{1}x}+c_{2}e^{m_{2}x}+\ldots+c_{n}e^{m_{n}x}$$

### Case 2: Real and Repeated Roots

$$y=c_{1}e^{m_{1}x}+c_{2}xe^{m_{1}x}+\dots+c_{n}x^{n-1}e^{m_{1}x}$$

where  

$$e^{m_1x}, xe^{m_1x}, \ldots, x^{n-1}e^{m_1x}$$

are `linearly independent`.[^4]

### Case 3: Complex Roots

- General solution when all roots are complex $n = 6$:

$$\begin{align}
   y &= e^{\alpha_1 x}(c_1 \cos \beta_1 x + c_2 \sin \beta_1 x)\\
   &+ e^{\alpha_2 x}(c_3 \cos \beta_2 x + c_4 \sin \beta_2 x)\\
   &+ e^{\alpha_3 x}(c_5 \cos \beta_3 x + c_6 \sin \beta_3 x)
   \end{align}
$$

- General solution when 4 roots are complex and 2 are real $n = 6$:

$$
\begin{align}
y &= e^{\alpha_1 x}(c_1 \cos \beta_1 x + c_2 \sin \beta_1 x)\\ 
&+ e^{\alpha_2 x}(c_3 \cos \beta_2 x + c_4 \sin \beta_2 x)\\
&+ c_5 e^{m x} + c_6 x e^{m x}
\end{align}
$$

- Complex root of multiplicity $k$:  
   If $m_1 = \alpha + \iota\beta$ is a root of multiplicity $k$, its `conjugate` $m_2 = \alpha - \iota\beta$ is also of multiplicity $k$.
   - General solution involves:  

   $$e^{(\alpha + i\beta)x}, \, x e^{(\alpha + i\beta)x}, \, x^2 e^{(\alpha + i\beta)x}, \, \dots, x^{k-1} e^{(\alpha + i\beta)x}$$

$$e^{(\alpha - i\beta)x}, \, x e^{(\alpha - i\beta)x}, \, x^2 e^{(\alpha - i\beta)x}, \, \dots, x^{k-1} e^{(\alpha - i\beta)x}$$

- General solution (using `Euler's formula`):  

$$y = e^{\alpha x} \left[ \sum_{n=0}^{k-1} c_n x^n \cos \beta x + \sum_{n=0}^{k-1} d_n x^n \sin \beta x \right]$$

- Example for $k = 3$:  

$$y = e^{\alpha x} \left[ (c_1 + c_2 x + c_3 x^2) \cos \beta x + (d_1 + d_2 x + d_3 x^2) \sin \beta x \right]$$

## Solving the `Auxiliary Equation`

## Solving the Auxiliary Equation

1. The auxiliary equation is:  

   $$ P_n(m) = 0, \quad n > 2 $$

2. To solve, guess a root $m_1$. Then, $m - m_1$ is a factor of $P_n(m)$.

3. By synthetic or regular division, factorize:  

   $$ P_n(m) = (m - m_1) Q(m) $$

4. Solve the quotient polynomial equation:  

   $$ Q(m) = 0 $$

5. If $m_1 = \frac{p}{q}$ is a rational root of $P_n(m)$, then:
   - $p$ is a factor of $a_0$ (constant term).
   - $q$ is a factor of $a_n$ (leading coefficient).

6. Use this fact to construct a list of all possible rational roots and test each using synthetic division.

### Example

$$y^{\prime\prime\prime} + 3y^{\prime\prime} - 4y = 0$$

#### Solution

$$y = e^{mx}$$

Then,  

$$y' = me^{mx}, y'' = m^2e^{mx}, \text{ and } y''' = m^3e^{mx}$$

Substituting this in the given differential equation, we have  

$$(m^3 + 3m^2 - 4)e^{mx} = 0$$

Since $e^{mx} \neq 0$, therefore  

$$m^3 + 3m^2 - 4 = 0$$

So that the auxiliary equation is  

$$m^3 + 3m^2 - 4 = 0$$

Solution of the `auxiliary equation`:  
If we take $m = 1$, then we see that  

$$m^3 + 3m^2 - 4 = 1 + 3 - 4 = 0$$

Therefore $m = 1$ satisfies the auxiliary equation so that $m - 1$ is a factor of the polynomial $m^3 + 3m^2 - 4$.

By synthetic division, we can write  

$$m^3 + 3m^2 - 4 = (m - 1)(m^2 + 4m + 4)$$

or  

$$m^3 + 3m^2 - 4 = (m - 1)(m + 2)^2$$

Therefore  

$$m^3 + 3m^2 - 4 = 0$$

$$\Rightarrow (m - 1)(m + 2)^2 = 0$$

$$\Rightarrow m = 1, -2, -2$$

Hence solution of the differential equation is  

$$y = c_1e^x + c_2e^{-2x} + c_3xe^{-2x}$$

## References

Read more about [[M_Notations|notations and symbols]].

[^1]: Read more about [[mth401_13|linear dependence]].
[^2]: Read more about [[mth401_14|solutions to higher order differential equations]].
[^3]: Read more about [[mth401_04|homogeneous differential equations]].
[^4]: Read more about [[mth401_07|linear differential equation]].