---
tags:
  - university-notes
university-name: Virtual University of Pakistan
date: 2024-11-28
---

# 15. Construction of a Second Solution

<span style="color: gray;">Dated: 28-11-2024</span>

## General case

Consider the differential equation  

$$a_{2}(x)\frac{d^{2}y}{dx^{2}}+a_{1}(x)\frac{dy}{dx}+a_{0}(x)y=0$$

Divide the above equation by $a_2(x)$ to convert this into the form  

$$y^{\prime\prime}+P(x)y'+Q(x)y=0$$

Where $P(x)$ and $Q(x)$ are `continuous`[^1] on the `interval`[^2] $I$.  
Suppose that $y_1(x) \ne 0, \forall x \in I$ is a solution to the above `differential equation` then

$$y_1^{\prime\prime}+P(x)y_1'+Q(x)y_1=0$$

We define $y = u(x) y_1(x)$ then  

$$y^\prime = uy^\prime_1 + y_1u^\prime$$

$$y^{\prime\prime} = uy^{\prime\prime}_1 + 2y^{\prime}_1u^{\prime} + y_1u^{\prime\prime}$$

$$y^{\prime\prime} + Py^\prime + Qy = u(y_1^{\prime\prime} + Py_1^\prime + Qy_1) + y_1u^{\prime\prime} + (2 y_1^\prime + Py_1)u^\prime = 0$$

$$\because y_1^{\prime\prime}+P(x)y_1'+Q(x)y_1=0$$

$$\therefore y_1u^{\prime\prime} + (2 y_1^\prime + Py_1)u^\prime = 0$$

Suppose $w = u^\prime$, then  

$$y_1w^\prime + (2y_1^\prime + Py_1)w = 0$$

Separating the variables, we have  

$$\frac {dw}{w} + \left(2 \frac {y_1^\prime}{y_1} + P\right)dx = 0$$

`Integrating`[^3] it  

$$ \ln|w| + 2\ln|y_1| = -\int Pdx + c $$

$$ \ln|w(y_1)^2| = -\int Pdx + c $$

$$ w(y_1)^2 = c_1e^{-\int Pdx} $$

$$ w = \frac{c_1e^{-\int Pdx}}{(y_1)^2} $$

$$\because w = u^\prime$$

$$ u^\prime = \frac{c_1e^{-\int Pdx}}{(y_1)^2} $$

Therefore, we `integrate`[^3] again.  

$$u = c_1\int \frac{e^{-\int Pdx}}{(y_1)^2}dx + c_2$$

$$\therefore y = u(x)y_{1}(x) = c_{1}y_{1}(x)\int\frac{e^{-\int Pdx}}{y_{1}^{2}}dx + c_{2}y_{1}(x)$$

Choosing $c_1 = 1$ and $c_2 = 0$, we obtain  

$$y_{2}=y_{1}(x)\int\frac{e^{-\int Pdx}}{(y_{1})^{2}}dx$$

## The Woolskin

$$W(y_1(x), y_2(x)) = 
\begin{vmatrix}
	y_1 & y_1 \int{\frac{e^{- \int Pdx}}{(y_1)^2}dx} \\
	(y_1)^\prime & \frac{e^{-\int Pdx}}{y_{1}}+y_{1}^{\prime}\int\frac{e^{-\int Pdx}}{{y_{1}}^{2}}dx
\end{vmatrix}
$$

$$= e^{- \int P dx} \ne 0, \forall x$$

Therefore, $y_1(x)$ and $y_2(x)$ are `linearly independent`[^4] and the `general solution`[^5] is  

$$y(x) = c_1y_1(x) + c_2y_2(x)$$

## Example

Given that  

$$y_1 = x^2$$

is a solution of  

$$x^2y^{\prime\prime} - 3xy^{\prime} + 4y = 0$$

Find the `general solution`[^5] of the differential equation on the `interval`[^2] $(0, \infty)$.

### Solution

The equation can be written as  

$$y''-\frac{3}{x}y'+\frac{4}{x^{2}}y=0$$

The second solution $y_2$ is given by  

$$y_{2}=y_{1}(x)\int\frac{e^{-\int Pdx}}{y_{1}^{2}}dx$$

$$y_{2}=x^{2}\int\frac{e^{\int\frac{3}{x}dx}}{x^{4}}dx=x^{2}\int\frac{e^{\ln x^{3}}}{x^{4}}dx$$

$$y_{2}=x^{2}\int\frac{1}{x}dx=x^{2}\ln x$$

Hence the `general solution`[^5] is  

$$y = c_1x^2 + c_2x^2 \ln (x)$$

## Order Reduction

Given that  

$$y_1 = x^3$$

is the solution of differential equation  

$$x^2y^{\prime\prime} - 6y = 0$$

Find the second solution of the equation

### Solution

Rewrite the equation into  

$$y^{\prime\prime}-\frac{6}{x^{2}}y=0$$

So that  

$$P(x)=-\frac{6}{x^{2}}$$

$$y_{2}=y_{1}\int\frac{e^{-\int Pdx}}{y_{1}^{2}}dx$$

$$y_{2}=x^{3}\int\frac{e^{-\int \frac{6}{x^{2}}dx}}{x^{6}}dx$$

$$y_{2}=x^{3}\int\frac{e^{\frac{6}{x}}}{x^{6}}dx$$

Therefore, using the formula  

$$y_{2}=y_{1}\int\frac{e^{-\int Pdx}}{(y_{1})^{2}}dx$$

This `integral`[^3] is hard to find therefore, we use an alternative approach.  
Let  

$$y = u(x)y_1(x)$$

$$y = u(x)x^3$$

Then  

$$y^{\prime}=3x^{2}u+x^{3}u^{\prime}$$

$$y^{\prime\prime}=x^3u^{\prime\prime}+6x^2u^\prime+6xu$$

Therefore  

$$x^{2}y^{\prime\prime}-6y=0$$

$$x^2(x^3u^{\prime}+6x^2u^{\prime}+6xu)-6ux^3=0$$

$$x^5u^{\prime\prime}+6x^4u^\prime=0$$

$$u^{\prime\prime}+\frac{6}{x}u^\prime=0$$

Then if we take $w = u^\prime$

$$w^\prime + \frac 6 x w = 0$$

Finding the `integrating factor`[^6]  

$$u(x)=e^{\int \frac{1}{x}dx}=e^{6\ln x}=x^{6}$$

Therefore  

$$x^6w'+6x^5w=0$$

$$\frac{d}{dx}(x^6w)=0$$

After `integration`,[^3] we have  

$$x^6w=c_1$$

$$u'=\frac{c_1}{x^6}$$

`Integrating`[^3] again  

$$u=-\frac{c_{1}}{5x^{5}}+c_{2}$$

$$y=ux^{3}=\frac{-c_{1}}{5x^{2}}+c_{2}x^{3}$$

Choosing $c_2 = 0$ and $c_1 = -5$, we obtain the second solution

$$y_2 = \frac 1 {x^2}$$

Hence the `general solution`[^5] is  

$$y=c_{1}x^{3}+c_{2}\left(\frac{1}{x^{2}}\right)$$

## References

Read more about [[M_Notations|notations and symbols]].

[^1]: Read more about [[mth101_12|continuity]].
[^2]: Read more about [[mth101_01|intervals]].
[^3]: Read more about [[mth101_25|integration]].
[^4]: Read more about [[mth401_13|linear dependence]].
[^5]: Read more about [[mth401_14|general solution]].
[^6]: Read more about [[mth401_06|integrating factor]].