---
tags:
  - university-notes
university-name: Virtual University of Pakistan
date: 2025-04-08
---

# Lecture No. 16

<span style="color: gray;">Dated: 08-04-2025</span>

Expression: `2 + 4 * 6`  
Output trace:

```
>> Expr::isPresent()
    >> Term::isPresent()
        >> Factor::isPresent() token: 2 (257) 
        << Factor::isPresent() return true
        >> Tprime::isPresent() token: + (267)
        << Tprime::isPresent() return false
    << Term::isPresent() return true
    >> Eprime::isPresent() token: + (267) 
        >> Term::isPresent()
            >> Factor::isPresent() token: 4 (257) 
            << Factor::isPresent() return true 
            >> Tprime::isPresent() token: * (269) 
                >> Factor::isPresent() token: 6 (257) 
                << Factor::isPresent() return true
                >> Tprime::isPresent() token: (0)
                << Tprime::isPresent() return false
            << Tprime::isPresent() return true
        << Term::isPresent() return true
        >> Eprime::isPresent() token: (0)
        << Eprime::isPresent() return false
    << Eprime::isPresent() return true
<< Expr::isPresent() return true
```

```
2 + 4 * 6
```

![[cs606_e_16_1.svg]]

## Non Recursive Predictive Parsing

This is done by maintaining an explicit `stack` and using a `table`.  
Such a `parser`[^1] is called `table driven parser`.  
The `LL(1) table` has one dimension for current `non-terminal` to expand and another dimension for next `token`.[^2] Each table cell contains one `production`.

### Example

#### Expression Grammar

```
1. E  ?   T E'
2. E' ? + T E'
3.    |   e
4. T  ?   F T'
5. T' ? * F T'
6.    | e
7. F  ? (E)
8.    | id
```

#### Predictive Parsing Table

|     | `id`         | `+`            | `*`            | `(`           | `)`           | `$`          |
|-----|--------------|----------------|----------------|---------------|---------------|--------------|
| `E` | `E → TE'`    |                |                | `E → TE'`     |               |              |
| `E'`|              | `E' → +TE'`    |                |               | `E' → ε`      | `E' → ε`     |
| `T` | `T → FT'`    |                |                | `T → FT'`     |               |              |
| `T'`|              | `T' → ε`       | `T' → *FT'`    |               | `T' → ε`      | `T' → ε`     |
| `F` | `F → id`     |                |                | `F → (E)`     |               |              |

The `predictive parser` uses an explicit `stack` to keep track of pending `non-terminals`. It can thus be implemented without `recursion`.

## $LL(1)$ Parsing Algorithm

Input `string`[^3] (`$` denoting the end of it), is contained inside an `input buffer`.  
Initially, the `stack` contains the starting symbol.

### Functionality

Consider

- Symbol at top of stack be `X`
- Current input symbol be `a`

There are 3 possibilities.

1. $X = a = \$$, the `parser`[^1] halts and announces successful completion.
2. $X = a \ne \$$, the `parser`[^1] pops $X$ and advances the input pointer to next input symbol.
3. If $X$ is `non terminal` then we consult $M[X, a]$ entry of the $M$ `table`.
	- If $M[X, a] = \{X ? UVW\}$ (a production), the `parser`[^1] replaces $X$ by $WVU$ ($U$ being at the top).
	- If $M[X, a] = \text{error}$ then the `parser`[^1] calls an error recovery routine.

### Example

Input `string`[^3]  

$$\text{id} + \text{id} \, \text{id}$$

| Stack           | Input         | Output           |
|----------------|---------------|------------------|
| $E             | id+idid$      | E → TE'          |
| $E' T          | id+idid$      | T → FT'          |
| $E' T' F       | id+idid$      | F → id           |
| $E' T'         | +idid$        |                  |
| $E'            | +idid$        | T' → ε           |
| $E'            | +idid$        | E' → +TE'        |
| $E' T +        | idid$         |                  |
| $E' T' F       | idid$         | T → FT'          |
| $E' T'         | id$           |                  |
| $E'            | id$           | T' → ε           |
| $E'            | id$           | E' → +TE'        |
| $E' T +        | id$           |                  |
| $E' T' F       | id$           | T → FT'          |
| $E' T'         | $             |                  |
| $E'            | $             | T' → ε           |
| $              | $             | E' → ε           |

## References

[^1]: Read more about [[cs606_02|parsers]].
[^2]: Read more about [[cs606_05|tokens]].
[^3]: Read more about [[cs402_01|strings]].