---
tags:
  - university-notes
university-name: Virtual University of Pakistan
date: 2025-03-01
---

# Lecture No. 25

<span style="color: gray;">Dated: 01-03-2025</span>

## Theorem

### Statement

If $L_1$ and $L_2$ are two `regular languages`[^1] then $L_1 \cap L_2$ is also a `regular language`.[^1]

### Proof

Using `De Morgan's` law  

$$(L_1^c \, \cup \, L_2^c)^c = (L_1^c)^c \, \cup \, (L_2^c)^c = L_1 \, \cap \, L_2$$

### Example

$$L_1 = \text{language of words with double a's}$$

$$L_2 = \text{language of words with even number of a's}$$

![[cs402_e_25_1.svg]]  
/// caption  
`Finite Automaton`[^2] for $L_1$.  
///

![[cs402_e_25_2.svg]]  
/// caption  
`Finite Automaton`[^2] for $L_2$.  
///  

$$r_1 = (a + b)^* aa (a + b)^*$$

$$r_2 = (b + ab^*a)^*$$

![[cs402_e_25_3.svg]]  
/// caption  
`Finite Automaton`[^2] for $L_1^c$.  
///  

![[cs402_e_25_4.svg]]  
/// caption  
`Finite Automaton`[^2] for $L_2^c$.  
///  

| Old States              | New States After Reading |                     |
| ----------------------- | ------------------------ | ------------------- |
|                         | a                        | b                   |
| $z_1 \pm \equiv (p, 1)$ | $(q, 2) \equiv z_4$      | $(p, 1) \equiv z_1$ |
| $z_2 + \equiv (p, 2)$   | $(q, 1) \equiv z_3$      | $(p, 2) \equiv z_2$ |
| $z_3 + \equiv (q, 1)$   | $(r, 2) \equiv z_6$      | $(p, 1) \equiv z_1$ |
| $z_4 + \equiv (q, 2)$   | $(r, 1) \equiv z_6$      | $(p, 2) \equiv z_2$ |
| $z_5 \equiv (r, 1)$     | $(r, 2) \equiv z_6$      | $(r, 1) \equiv z_6$ |
| $z_6 + \equiv (r, 2)$   | $(r, 1) \equiv z_5$      | $(r, 2) \equiv z_6$ |

![[cs402_e_25_5.svg]]  
/// caption  
`Finite Automaton`[^2] for $L_1^c \, \cup \, L_2^c$.  
///  

![[cs402_e_25_6.svg]]  
/// caption  
`Finite Automaton`[^2] for $L_1 \, \cap \, L_2$.  
///  

## References

[^1]: Read more about [[CS402_04|regular languages]].
[^2]: Read more about [[cs402_04|finite automaton]].