---
tags:
  - university-notes
  - differentiation
  - partial-differential
university-name: Virtual University of Pakistan
date: 2024-10-30
---

<span style="color: gray;">Dated: 30-10-2024</span>

# Geometric Meaning of Partial Derivative

## Geometric Meaning of `partial derivative`[^1]

Imagine we have  

$$z = f(x, y)$$

then the `partial derivative`[^1] with respect to $x$ is denoted by  

$$\frac{\partial z}{\partial x}$$

$$f_x$$

$$\frac{\partial f}{\partial x}$$

and with respect to $y$, it is  

$$\frac{\partial z}{\partial y}$$

$$f_y$$

$$\frac{\partial f}{\partial y}$$

## Partial Derivatives

Let $z = f(x, y)$ be a `function`[^2] of $x$ and $y$, then keeping $y$ as a `constant`, change in $f(x, y)$ due to change if $x$ can be given by  

$$\Delta z = f(x + \Delta x, y) - f(x, y)$$

If the following ratio  

$$\frac{\Delta z}{\Delta x} = \frac{f(x + \Delta x, y) - f(x, y)}{\Delta x}$$

approaches to a `limit`[^3] $\Delta x \to 0$ then  

$$f_x(x, y) = \frac{\partial z}{\partial x} = \lim_{\Delta x \to 0} \frac{f(x + \Delta x, y) - f(x, y)}{\Delta x}$$

This is called `partial derivative`[^1] with respect to $x$.  
Similarly, the `partial derivative`[^1] with respect to $y$ will be

$$f_y(x, y) = \frac{\partial z}{\partial y} = \lim_{\Delta y \to 0} \frac{f(x, \Delta y + y) - f(x, y)}{\Delta y}$$

## Geometric Meaning of `partial derivative`[^1]

![[Pasted image 20241007203726.png]]

Imagine we have $z = f(x, y)$ being a `function`[^2] of 2 `variables` and its graph is a `surface`.  
Then the coordinates of any arbitrary point $P$ at $(x_0, y_0)$ are $P(x_0, y_0, f(x_0, z_0))$.  
And if this point starts moving on the `surface` such that $y$ remains `constant` then  
On this `curve`, $\frac{\partial z}{\partial x}$ is the `partial derivative`[^1] with respect to $x$ since $y$ is `constant`. This gives us the `tangent slope` to this `curve`. 

Similarly, for $y$, we have  
![[Pasted image 20241007204603.png]]

## Partial Derivatives of Higher Orders

$$\frac{\partial}{\partial x} \left(\frac{\partial f}{\partial x}\right) = \frac{\partial ^2 f}{\partial x^2} = \frac{\partial}{\partial x} f_x = f_{xx} = f_{x^2}$$

$$\frac{\partial}{\partial y} \left(\frac{\partial f}{\partial x}\right) = \frac{\partial ^2 f}{\partial y \partial x} = \frac{\partial}{\partial y} f_x = f_{xy}$$

$$\frac{\partial}{\partial x} \left(\frac{\partial f}{\partial y}\right) = \frac{\partial ^2 f}{\partial x \partial y} = \frac{\partial}{\partial x} f_y = f_{yx}$$

$$\frac{\partial}{\partial y} \left(\frac{\partial f}{\partial y}\right) = \frac{\partial ^2 f}{\partial y^2} = \frac{\partial}{\partial y} f_y = f_{yy} = f_{y^2}$$

The $f_{xy}$ and $f_{yx}$ are called `mixed second partials` and usually are not equal.  

### Example

$$ f(x, y) = x \cos y + y e^x $$

$$ \frac{\partial f}{\partial x} = \cos y + y e^x $$

$$ \frac{\partial^2 f}{\partial y \partial x} = \frac{\partial}{\partial y} \left( \frac{\partial f}{\partial x} \right) = -\sin y + e^x $$

$$ \frac{\partial^2 f}{\partial x^2} = \frac{\partial}{\partial x} \left( \frac{\partial f}{\partial x} \right) = y e^x $$

$$ f(x, y) = x \cos y + y e^x $$

$$ \frac{\partial f}{\partial y} = -x \sin y + e^x $$

$$ \frac{\partial^2 f}{\partial x \partial y} = -\sin y + e^x $$

$$ \frac{\partial^2 f}{\partial y^2} = \frac{\partial}{\partial y} \left( \frac{\partial f}{\partial y} \right) = -x \cos y $$

## Laplace's Equation

Let $w=f(x, y, z)$ be a `function`[^2] then  

$$\frac{\partial^2 f}{\partial x^2} + \frac{\partial^2 f}{\partial y^2} + \frac{\partial^2 f}{\partial z^2} = 0$$

It also works for `functions`[^2] of 2 `variables`.

## Euler's Theorem or Mixed Derivative Theorem

If $f(x, y)$ and its `partial derivatives`[^1] $f_x, f_y, f_{xy}$ and $f_{yx}$ are defined throughout an `open region` containing a point $(a, b)$ and are all `continuous`[^4] at $(a, b)$ then  

$$f_{xy}(a, b) = f_{yx}(a, b)$$

### Advantages

$$w = xy + \frac{e^y}{y^2 + 1}$$

The following suggests us to take `partial derivative`[^1] with respect to $y$ first and then with respect to $x$.  

$$\frac{\partial ^ 2 w}{\partial x \partial y}$$

Using the theorem, if we `partially derivate`[^1] with respect to $x$ first then finding the answer becomes more quicker.  

$$\frac{\partial w}{\partial x} = y$$

$$\frac{\partial^2 w}{\partial y \partial x} = 1$$

## References

Read more about [[M_Notations|notations and symbols]].

[^1]: Read more about [[semester 2/MTH301 - Calculus II/6. Geometry of continuous functions/Lecture|partial derivatives]].
[^2]: Read more about [[M_Function|functions]].
[^3]: Read more about [[9. Limits (Intuitive Introduction)|limits]].
[^4]: Read more about [[12. Continuity|continuity]].