---
tags:
  - university-notes
university-name: Virtual University of Pakistan
date: 2024-12-01
---

<span style="color: gray;">Dated: 01-12-2024</span>

# 18. Method of Undetermined Coefficients (Annihilator Operator Approach 1)

## Differential Operators

In `calculus`, we often denote $\frac d {dx}$ by $D$.  
This is known as `differential operator`.  
This operator possesses linearity, meaning if $f$ and $g$ are two differentiable functions then  

$$D(a f(x) + b g(x)) = aDf(x) + bDg(x)$$

Therefore, we call it `linear differential operator`.  

$$\frac{d^2y}{dx^2}=\frac{d}{dx}\left(\frac{dy}{dx}\right)=D(Dy)=D^2y$$

The following are also `linear differential operators`  

$$a_nD^n+a_{n-1}D^{n-1}+\cdots+a_1D+a_0$$

$$D+3, D^{2}+3D-4, 5D^{3}-6D^{2}+4D$$

## Differential Equation in terms of $D$

Any linear differential equation can be expressed in terms of the notation $D$. Consider a $2^{nd}$ order equation with constant coefficients

$$ay''+by'+cy=g(x)$$

Since

$$
\frac{dy}{dx}=Dy, \frac{d^2y}{dx^2}=D^2y
$$

Therefore the equation can be written as

$$
aD^2y+bDy+cy=g(x)
$$

or

$$
(aD^2 + bD + c)y = g(x)
$$

Now, we define another differential operator $L$ as

$$
L = aD^2 + bD + c
$$

Then the equation can be compactly written as

$$
L(y) = g(x)
$$

The operator $L$ is a second-order linear differential operator with constant coefficients.

### Example

Consider the differential equation

$$
y'' + y' + 2y = 5x - 3
$$

Since

$$
\frac{dy}{dx} = Dy, \quad \frac{d^2y}{dx^2} = D^2y
$$

Therefore, the equation can be written as

$$
(D^2 + D + 2)y = 5x - 3
$$

Now, we define the operator $L$ as

$$
L = D^2 + D + 2
$$

Then the given differential can be compactly written as

$$
L(y) = 5x - 3
$$

## Factorization of a Differential Operator

An $nth$ order linear differential operator  

$$L=a_nD^n+a_{n-1}D^{n-1}+\ldots+a_1D+a_0$$

with constant coefficients can be factorized, whenever the characteristics polynomial equation  

$$L=a_nm^n+a_{n-1}m^{n-1}+\ldots+a_1m+a_0$$

can be factorized.  
The factors of a linear differential operator with constant coefficients commute.

### Example

Consider the following $2^{nd}$ order linear differential operator

$$D^2 + 5D + 6$$

If we treat $D$ as an algebraic quantity, then the operator can be factorized as

$$D^2 + 5D + 6 = (D + 2)(D + 3)$$

To illustrate the commutative property of the factors, we consider a twice-differentiable function $y = f(x)$. Then we can write

$$(D^2 + 5D + 6)y = (D + 2)(D + 3)y = (D + 3)(D + 2)y$$

To verify this we let  

$$w=(D+3)y=y'+3y$$

Then

$$(D+2)w=Dw+2w$$

$$(D+2)w=(y''+3y')+(2y'+6y)$$

$$(D+2)w=y''+5y'+6y$$

or  

$$(D+2)(D+3)y=y''+5y'+6y$$

Similarly if we let  

$$w=(D+2)y=(y'+2y)$$

Then

$$(D+3)w=Dw+3w=(y''+2y')+(3y'+6y)$$

$$(D+3)w=y''+5y'+6y$$

$$(D+3)(D+2)y=y''+5y'+6y$$

Therefore, we can write from the two expressions that  

$$(D+3)(D+2)y=(D+2)(D+3)y$$

Hence  

$$(D+3)(D+2)y=(D+2)(D+3)y$$

## Annihilator Operator

Suppose that

- $L$ is a linear differential operator with constant coefficients.
- $y = f(x)$ defines a sufficiently differentiable function.
- The function $f$ is such that $L(y) = 0$

Then the differential operator $L$ is said to be an annihilator operator of function $f$.

### Example

Find a differential operator that annihilates the polynomial function

$$y=1-5x^{2}+8x^{3}.$$

#### Solution

Since  

$$D^{4}x^{3}=0$$

Therefore  

$$D^{4}y=D^{4}(1-5x^{2}+8x^{3})=0.$$

Hence, $D^4$ is the differential operator that annihilates the function $y$.

Note that the functions that are annihilated by an nth-order linear differential operator $L$ are simply those functions that can be obtained from the general solution of the homogeneous differential equation

$$L(y) = 0$$

## Notes

- If $y_1$ and $y_2$ are functions and $L(y_1) = 0$ and $L(y_2) = 0$.  

$$L\left(c_1y_1(x) + c_2y_2(x)\right) = 0$$

- Suppose $L_1$ and $L_2$ being linear operators with constant coefficients such that  

$$L_1(y_1) = 0, L_2(y_2) = 0$$

$$L_1(y_2) \ne 0, L_2(y_1) \ne 0$$

then  

$$L_1L_2(y_1(x) + y_2(x)) = 0$$

To demonstrate this fact we use the linearity property for writing

$$L_1L_2(y_1+y_2) = L_1L_2(y_1) + L_1L_2(y_2)$$

Since  

$$L_1L_2 = L_2L_1$$

therefore  

$$L_1L_2(y_1+y_2) = L_2L_1(y_1) + L_1L_2(y_2)$$

or  

$$L_1L_2(y_1+y_2) = L_2(L_1(y_1)) + L_1(L_2(y_2))$$

But we know that  

$$L_1(y_1) = 0, \quad L_2(y_2) = 0$$

Therefore  

$$L_1L_2(y_1 + y_2) = L_2(0) + L_1(0) = 0$$

### Example

Find a differential operator that annihilates the function

$$f(x)=7-x+6\sin{3x}$$

#### Solution

Suppose that

$$y_1(x)=7-x,\quad y_2(x)=6\sin{3x}$$

Then

$$D^2y_1(x)=D^2(7-x)=0$$

$$(D^2+9)y_2(x)=(D^2+9)\sin{3x}=0$$

Therefore, $D^2(D^2+9)$ annihilates the function $f(x)$.

## References

Read more about [[M_Notations|notations and symbols]].
