---
tags:
  - university-notes
university-name: Virtual University of Pakistan
date: 2024-12-01
---

<span style="color: gray;">Dated: 01-12-2024</span>

# 19. Method of Undetermined Coefficients (Annihilator Operator Approach 2)

This method is limited to non homogeneous linear differential equations with following factors

- Constant coefficients
- $g(x)$ has a specific form

## Form of $g(x)$

Any of the following are valid

- A constant function $k$.
- A polynomial function
- An exponential function
- The trigonometric functions $\sin (\beta x), \cos(\beta x)$
- Finite sums and products of these functions

## The Method

 - Write the non homogeneous linear differential equation in the form  

$$L(y) = g(x)$$

- Find the complementary solution $y_c$ by finding general solution of the associated homogeneous differential equation  

$$L(y) = 0$$

- Operate on both sides of the non homogeneous equation with a differential operator $L_1$ that annihilates the function $g(x)$.
- Find the general solution of the higher order homogeneous differential equation  

$$L_1L(y) = 0$$

- Delete all those terms from step 4 that are duplicated in $y_c$ found in step 2
- Form a linear combination $y_p$ of the terms that remain. This is the form of a particular solution of the non homogeneous differential equation  

$$L(y) = g(x)$$

- Substitute $y_p$ found in step 6 into the given non-homogeneous linear differential equation $L(y) = g(x)$. Match coefficients of various functions on each side of the equality and solve the resulting system of equations for the unknown coefficients in $y_p$.
- With the particular integral found in step 7, form the general solution of the given differential equation as  

$$y = y_c + y_p$$

## Example

Solve

$$\frac{d^{2}y}{dx^{2}}+3\frac{dy}{dx}+2y=4x^{2}.$$

### Solution

#### Step 1

since

$$\frac{dy}{dx}=Dy,\quad \frac{d^{2}y}{dx^{2}}=D^{2}y$$

Therefore, the given differential equation can be written as

$$(D^{2}+3D+2)y=4x^{2}$$

#### Step 2

To find the complementary function $y_{c}$, we consider the associated homogeneous differential equation

$$(D^{2}+3D+2)y=0$$

The auxiliary equation is 

$$m^{2}+3m+2=(m+1)(m+2)=0$$

$$\implies m=-1,-2$$

Therefore, the auxiliary equation has two distinct real roots.

$$m_{1}=-1,\quad m_{2}=-2$$

Thus, the complementary function is given by

$$y_{c}=c_{1}e^{-x}+c_{2}e^{-2x}$$

#### Step 3

In this case the input function is

$$g(x)=4x^{2}$$

Further  

$$D^{3}g(x)=4D^{3}x^{2}=0$$

Therefore, the differential operator $D^3$ annihilates the function $g$. Operating on both sides of the equation in step 1, we have

$$D^3(D^2+3D+2)y=4D^3x^2$$

$$D^3(D^2+3D+2)y=0$$

This is the homogeneous equation of order 5. Next we solve this higher order equation.

#### Step 4

The auxiliary equation of the differential equation in step 3 is

$$m^3(m^2+3m+2)=0$$

$$m^3(m+1)(m+2)=0$$

$$m=0,0,0,-1,-2$$

Thus its general solution of the differential equation must be

$$y=c_1+c_2x+c_3x^2+c_4e^{-x}+c_5e^{-2x}$$

#### Step 5

The following terms constitute $y_c$

$$c_4e^{-x}+c_5e^{-2x}$$

Therefore, we remove these terms and the remaining terms are

$$y=c_1+c_2x+c_3x^2$$

#### Step 6

This means that the basic structure of the particular solution $y_p$ is

$$y_p=A+Bx+Cx^2$$

Where the constants $c_1$, $c_2$, and $c_3$ have been replaced, with $A$, $B$, and $C$, respectively.

#### Step 7

Since

$$y_p=A+Bx+Cx^2$$

$$y_p'=B+2Cx$$

$$y_p''=2C$$

Therefore

$$y_p''+3y_p'+2y_p=2C+3B+6Cx+2A+2Bx+2Cx^2$$

$$y_p''+3y_p'+2y_p=(2C)x^2+(2B+6C)x+(2A+3B+2C)$$

Substituting into the given differential equation, we have

$$(2C)x^2+(2B+6C)x+(2A+3B+2C)=4x^2+0x+0$$

Equating the coefficients of $x^2$, $x$, and the constant terms, we have

$$2C=4$$

$$2B+6C=0$$

$$2A+3B+2C=0$$

Solving these equations, we obtain

$$A=7,\quad B=-6,\quad C=2$$

Hence  

$$y_p=7-6x+2x^2$$

#### Step 8

The general solution of the given non-homogeneous differential equation is

$$y=y_c+y_p$$

$$y=c_1e^{-x}+c_2e^{-2x}+7-6x+2x^2$$

## References

Read more about [[M_Notations|notations and symbols]].
