---
tags:
  - university-notes
university-name: Virtual University of Pakistan
date: 2024-11-10
---

# 07. First order Linear Equation

<span style="color: gray;">Dated: 10-11-2024</span>

The differential equation of the form  

$$a(x)\frac{dy}{dx}+b(x)y=c(x)$$

is the `linear differential equation` of first order.  
It can be re-written as  

$$\frac{dy}{dx}+p(x)y=q(x)$$

where $p(x)$ and $q(x)$ are `continuous functions`.[^1]

## Method of Solution

General solution is given by  

$$y=\frac{\int u(x)q(x)dx+C}{u(x)}$$

where the `integrating factor`[^2] $u(x)$ is  

$$u(x)=\exp\left(\int p(x)dx\right)$$

## Summary

- Identify the $1^{\text{st}}$ order `linear differential equation` and re-write in the form  

$$\frac{dy}{dx}+p(x)y=q(x)$$

- Find the `integrating factor`[^2] 

$$u(x)=e^{\int p(x)dx}$$

- Write the general equation  

$$y=\frac{\int u(x)q(x)dx+C}{u(x)}$$

- If given an `initial value problem`[^3] then use the initial condition to find the constant $C$.
- Plug in the calculated value to write the particular solution of the problem.

## Example

$$(x-1)^{3}\frac{dy}{dx}+4(x-1)^{2}y=x+1$$

### Step 1

$$\frac{dy}{dx}+\frac{4}{x-1}y=\frac{x+1}{(x-1)^{3}}$$

$$P(x)=\frac{4}{x-1}$$

### Step 2

$$u(x) = \exp\left[\int \frac{4}{x-1}dx\right]$$

$$=\exp[\ln(x-1)^{4}]$$

$$=(x-1)^{4}$$

### Step 3

$$(x-1)^{4}\frac{dy}{dx}+4(x-1)^{3}y=x^{2}-1$$

$$\frac{d}{dx}[y(x-1)^{4}]=x^{2}-1$$

$$y(x-1)^{4}=\frac{x^{3}}{3}-x+c$$

## References

Read more about [[M_Notations|notations and symbols]].

[^1]: Read more about [[12. Continuity|continuity]].
[^2]: Read more about [[MTH401_06|integrating factor]].
[^3]: Read more about [[MTH401_02|initial value problem]].