---
tags:
  - university-notes
university-name: Virtual University of Pakistan
date: 2025-08-16
---

# 08. Muller’s Method

<span style="color: gray;">Dated: 16-08-2025</span>

## Example

Do two iterations of `Muller`’s method to solve $x^3 - 3x + 1 = 0$ starting with $x_0 = 0.5, x_2 = 0, x_1 = 1$ 

### Solution

$$f(x_0) = f_0 = (0.5)^3 - 3(0.5) + 1 = -0.375$$

$$f(x_1) = f_1 = (1)^3 - 3(1) + 1 = -1$$

$$f(x_2) = f_2 = 0 - 3 \times 0 + 1 = +1$$

$$c = f_0 = -0.375$$

$$h_1 = x_1 - x_0 = 0.5$$

$$h_2 = x_0 - x_2 = 0.5$$

$$a = \frac{h_2 f_1 - (h_1 + h_2)f_0 + h_1 f_2}{h_1 h_2 (h_1 + h_2)} = \frac{(0.5)(-1) - (-0.375) + (0.5)}{0.25} = 1.5$$

$$b = \frac{f_1 - f_0 - ah_1^2}{h_1} = -2$$

$$\therefore x = x_0 - \frac{2c}{+b - \sqrt{b^2 - 4ac}} = 0.5 - \frac{2(-0.375)}{-2 - \sqrt{4 + 4(1.5)(0.375)}} = 0.5 - \frac{-0.75}{-2 - \sqrt{4 + 2.25}} = 0.33333 < 0.5$$

Take  

$$x_0 = 0.\overline{3}, \quad x_1 = 0.5, \quad x_2 = 0$$

$$h_1 = x_1 - x_0 = 0.16667, \quad h_2 = x_0 - x_2 = 0.\overline 3$$

$$c = f_0 = f(0.\overline 3)$$

$$= x_0^3 - 3x_0 + 1 = 0.037046$$

$$f_1 = x_1^3 - 3x_1 + 1 = - 0.375$$

$$f_2 = x_2^3 - 3x_2 + 1 = 1$$

$$a = \frac{h_2 f_1 - (h_1 + h_2)f_0 + h_1 f_2}{h_1 h_2 (h_1 + h_2)} = \frac{0.023148}{0.027778} = 0.8333$$

$$b = \frac{f_1 - f_0 - ah_1^2}{h_1} = -2.6$$

$$x = x_0 - \frac{2c}{b - \sqrt{b^2 - 4ac}} = 0.333333 - \frac{0.074092}{-5.2236} = 0.3475 > 0.333333 = x_0$$

For 3rd iteration, we take  

$$x_0 = 0.3475, \quad x_1 = 0.5, \quad x_2 = 0.\overline 3$$

## Graeffe’s Root Squaring Method

This one is for 3rd degree `polynomial`[^1]

$$f(x) = a_0 + a_1 x + a_2 x^2 + a_3 x^3$$

$$f(-x) = a_0 - a_1 x + a_2 x^2 - a_3 x^3$$

$$f(x)f(-x) = a_3^2 x^6 - (a_2^2 - 2a_1 a_3)x^4 + (a_1^2 - 2a_0 a_2)x^2 - a_0^2$$

$$f(x)f(-x) = a_3^2 t^3 - (a_2^2 - 2a_1 a_3)t^2 + (a_1^2 - 2a_0 a_2)t - a_0^2 \quad \text{where } t = x^2$$

Suppose, we have squared the given `polynomial`[^1] $i$ times, then we can estimate the value of the roots by evaluating $2i$ `root`[^2] of  

$$\left| \frac{a_i}{a_{i-1}} \right|, \quad i=1,2,\dots,n$$

Where $n$ is the `degree` of the `polynomial`.[^1]

> [!NOTE] The proper sign of each `root`[^2] can be determined by recalling the original equation. This method fails, when the `roots`[^2] of the given `polynomial`[^1] are repeated.  

$$f(x) = x^n + a_1 x^{n-1} + a_2 x^{n-2} + \dots + a_{n-1}x + a_n$$

$$\left(x^n + a_2 x^{n-2} + a_4 x^{n-4} + \dots\right)^2 = \left(a_1 x^{n-1} + a_3 x^{n-3} + a_5 x^{n-5} + \dots\right)^2$$

Putting $x^2 = y$ and after simplifying, we have

$$y^n + b_1 y^{n-1} + b_1 y^{n-1} + \dots + b_1 y^{n-1} + b_n = 0$$

$$
\begin{aligned}
	b_1 &= -a_1^2 + 2a^2 \\
	b_2 &= a_2^2 - 2a_1 a_3 + 2a_4 \\
	\cdots &= \cdots \\
	b_n &= (-1)^n a_n^2
\end{aligned}
$$

## Example

Using `Graeffe root squaring method`, find all the `roots`[^2] of the equation

$$x^3 - 6x^2 + 11x - 6 = 0$$

### Solution

Using `Graeffe root squaring method`, the first three squared `polynomials`[^1] are as under  
For $i = 1$, the `polynomial`[^1] is  

$$x^3 - (36 - 22)x^2 + (121 - 72)x - 36 = x^3 - 14x^2 + 49x - 36$$

For $i = 2$, the `polynomial`[^1] is  

$$x^3 - (196 - 98)x^2 + (2401 - 1008)x - 1296 = x^3 - 98x^2 + 1393x - 1296$$

For $i = 3$, the `polynomial`[^1] is  

$$x^3 - (9604 - 2786)x^2 + (1940449 - 254016)x - 1679616 = x^3 - 6818x^2 + 1686433x - 1679616$$

The `roots`[^2] of `polynomial`[^1] are

$$\sqrt{\frac{36}{49}} = 0.85714, \quad \sqrt{\frac{49}{14}} = 1.8708, \quad \sqrt{\frac{14}{1}} = 3.7417$$

Similarly the `roots`[^2] of the `polynomial`[^1] are

$$\sqrt[4]{\frac{1296}{1393}} = 0.9821, \quad \sqrt[4]{\frac{1393}{98}} = 1.9417, \quad \sqrt[4]{\frac{98}{1}} = 3.1464$$

$$\sqrt[8]{\frac{1679616}{1686433}} = 0.99949, \quad \sqrt[8]{\frac{1686433}{6818}} = 1.99143, \quad \sqrt[8]{\frac{6818}{1}} = 3.0144$$

The exact values of the `roots`[^2] of the given `polynomial`[^1] are $1, 2$ and $3$.

## References

Read more about [[M_Notations|notations and symbols]].

[^1]: Read more about [[mth101_01|polynomials]].
[^2]: Read more about [[mth603_03|roots of an equation]].