---
tags:
  - university-notes
university-name: Virtual University of Pakistan
date: 2025-08-16
---

# 09. Solution of Linear System of Equations (`Gaussian Elimination` Method)

<span style="color: gray;">Dated: 16-08-2025</span>

The solution of the system of equations gives $n$ unknown values $x_1, x_2, \ldots, x_n$, which satisfy the system simultaneously. If $m > n$, the system usually will have an infinite number of solutions.

If $|A| \ne 0$ then the system has a unique solution, otherwise, there is no solution.

Under elimination methods, we consider

- `Gaussian elimination` 
- `Gauss-Jordan elimination`

> [!NOTE] `Crout’s reduction` also known as `Cholesky’s reduction` is considered under decomposition methods.

## Gaussian Elimination Method

### Stages

- The given system of equations is reduced to an equivalent `upper triangular`[^1] form using `elementary transformations`.[^2]
- the `upper triangular`[^1] system is solved using back `substitution procedure`.

$$
\begin{aligned}
	a_{11}x_1 + a_{12}x_2 + &\cdots + a_{1n}x_n = b_1 \\
	a_{21}x_1 + a_{22}x_2 + &\cdots + a_{2n}x_n = b_2 \\
	&\vdots \\
	a_{n1}x_1 + a_{n2}x_2 + &\cdots + a_{nn}x_n = b_n \\
\end{aligned}
$$

#### Stage 1

Substituting the value of $x_1$ from first equation into the rest

$$
\begin{aligned}
	x_1 + a_{12}^\prime x_2 + &\cdots + a_{1n}^\prime x_n = b_1^\prime \\
	a_{22}^\prime x_2 + &\cdots + a_{2n}^\prime x_n = b_2^\prime \\
	&\vdots \\
	a_{n2}^\prime x_2 + &\cdots + a_{nn}^\prime x_n = b_n^\prime \\
\end{aligned}
$$

Now, $x_1$ is eliminated for $(n - 1)^{th}$ equations, making them independent of $x_1$.  
Repeat the same process for $x_2, x_3, \ldots, x_{n - 1}$.  
This will get us the following `upper triangular form`.[^1]

$$
\left.
\begin{aligned}
	c_{11} x_1 + c_{12} x_2 + \cdots c_{1n} x_n &= d_1 \\
	c_{22} x_2 + \cdots c_{2n} x_n &= d_2 \\
	&\vdots \\
	c_{nn} x_n &= d_n
\end{aligned}
\right\}
$$

#### Stage 2

The values of the unknowns are determined by `backward substitution`. First $x_n$ is found from the last equation and then substitution this value of $x_n$ in the preceding equation will give the value of $x_{n-1}$. Continuing this way, we can find the values of all other unknowns

## Example

Solve the following system of equations using `Gaussian elimination` method

$$
\begin{aligned}
	2x + 3y - z &= 5 \\
	4x + 4y - 3z &= 3 \\
	-2x + 3y - z &= 1
\end{aligned}
$$

### Solution

#### Stage 1

$$
\begin{aligned}
	2x + 3y - z &= 5 \\
	4x + 4y - 3z &= 3 \\
	-2x + 3y - z &= 1
\end{aligned}
$$

$$
\left \downarrow 
\begin{aligned}
	\text{eq}_2 = \text{eq}_2 - \frac{\text{eq}_1}{2} \\
	\text{eq}_3 = \text{eq}_3 - \frac{\text{eq}_1}{2} \\
\end{aligned}
\right.
$$

$$
\begin{aligned}
	x + \frac 3 2 y - \frac z 2 &= \frac 5 2\\
	3x + \frac 5 2 y - \frac 5 2 z &= \frac 1 2 \\
	-3x + \frac 3 2 y - \frac z 2 &= -\frac 3 2
\end{aligned}
$$

$$
\left \downarrow 
\begin{aligned}
	\text{eq}_2 = \text{eq}_2 - 3 \times \text{eq}_1\\
	\text{eq}_3 = \text{eq}_3 + 3 \times \text{eq}_1 \\
\end{aligned}
\right.
$$

$$
\left.
\begin{aligned}
	x + \frac 3 2 y - \frac z 2 &= \frac 5 2\\
	- 2 y - z &= -7 \\
	6 y - 2 z &= 6
\end{aligned}
\right\}
$$

$$
\left \downarrow 
\begin{aligned}
	\text{eq}_2 = \frac {\text{eq}_2}{-2}\\
\end{aligned}
\right.
$$

$$
\begin{aligned}
	x + \frac 3 2 y - \frac z 2 &= \frac 5 2\\
	y + \frac z 2 &= \frac 7 2 \\
	6 y - 2 z &= 6
\end{aligned}
$$

$$
\left \downarrow 
\begin{aligned}
	\text{eq}_3 = \text{eq}_3 - 6 \times \text{eq}_2\\
\end{aligned}
\right.
$$

$$
\left.
\begin{aligned}
	x + \frac 3 2 y - \frac z 2 &= \frac 5 2\\
	y + \frac z 2 &= \frac 7 2 \\
	5 z &= -15
\end{aligned}
\right\}
$$

#### Stage 2

$$z = 3$$

$$\implies y = \frac{7}{2} - \frac{3}{2} = 2$$

$$\implies x = \frac{5}{2} + \frac{3}{2} - 3 = 1$$

Therefore, solution is $(1, 2, 3)$.

## Partial and Full Pivoting

The `Gaussian elimination` method fails if any one of the `pivot`[^3] elements becomes `zero`. In such a situation, we rewrite the equations in a different order to avoid zero `pivots`.[^3] Changing the order of equations is called `pivoting`.

> [!NOTE] In `partial pivoting`, only the rows are interchanged but in `full pivoting`, rows _and_ columns are interchanged.

A `linear system`[^4] of $m$ equations can be written as $n$ unknowns $x_1, x_2, \ldots, x_n$.

$$
A = \begin{bmatrix}
	a_{11} & a_{12} & a_{13} & \dots & a_{1n} \\
	a_{21} & a_{22} & a_{23} & \dots & a_{2n} \\
	\vdots & \vdots & \vdots & \ddots & \vdots \\
	a_{m1} & a_{m2} & a_{m3} & \dots & a_{mn}
\end{bmatrix} \\
\begin{bmatrix}
	x_1 \\
	x_2 \\
	\vdots \\
	x_n
\end{bmatrix} \\
=
\begin{bmatrix}
	b_1 \\
	b_2 \\
	\vdots \\
	b_m
\end{bmatrix} \\
$$

## Example

Solve the system of equations by `Gaussian elimination method` with [partial pivoting](#partial-and-full-pivoting).

$$
\begin{aligned}
	x+y+z &= 7 \\
	3x+3y+4z &= 24 \\
	2x+y+3z &= 16
\end{aligned}
$$

$$
\begin{bmatrix}
	1 & 1 & 1 \\
	3 & 3 & 4 \\
	2 & 1 & 3
\end{bmatrix}
\begin{bmatrix}
	x \\
	y \\
	z
\end{bmatrix}
=
\begin{bmatrix}
	7 \\
	24 \\
	16
\end{bmatrix}
$$

However, a glance at the first column reveals that the numerically largest element is $3$ which is in second row.  
Interchanging first 2 rows, we have.

$$
\begin{bmatrix}
	3 & 3 & 4 \\
	1 & 1 & 1 \\
	2 & 1 & 3
\end{bmatrix}
\begin{bmatrix}
	x \\
	y \\
	z
\end{bmatrix}
=
\begin{bmatrix}
	24 \\
	7 \\
	16
\end{bmatrix}
$$

### Stage 1

$$
\begin{bmatrix}
	1 & 1 & \frac{4}{3} \\
	0 & -1 & \frac{1}{3} \\
	0 & 0 & -\frac{1}{3}
\end{bmatrix}
\begin{bmatrix}
	x \\
	y \\
	z
\end{bmatrix}
=
\begin{bmatrix}
	8 \\
	0 \\
	-1
\end{bmatrix}
$$

### Stage 2

$$z = 3$$

$$\implies y = 1$$

$$\implies x = 3$$

# References

Read more about [[M_Notations|notations and symbols]].

[^1]: Read more about [[mth501_17|triangular matrices]].
[^2]: Read more about [[mth501_03|elementary row operations]].
[^3]: Read more about [[mth501_04|pivots]].
[^4]: Read more about [[mth501_03|linear systems]].