---
tags:
  - university-notes
university-name: Virtual University of Pakistan
date: 2025-08-18
---

# 10. Solution of Linear System of Equations(Gauss–Jordon Elimination Method)

<span style="color: gray;">Dated: 18-08-2025</span>

## Gauss–Jordon Elimination Method

This is the variation of `Gaussian elimination method`[^1] in which the given `linear system`[^2] is reduced to `diagonal`[^3] form.

### Example

$$
\left.
\begin{aligned}
	x+2y+z &=8 \\
	2x+3y+4z &=20 \\
	4x+3y+2z &=16
\end{aligned}
\right\}
$$

$$
\begin{bmatrix}
	1 & 2 & 1 \\
	2 & 3 & 4 \\
	4 & 3 & 2
\end{bmatrix}
\begin{bmatrix}
	x \\
	y \\
	z
\end{bmatrix}
=
\begin{bmatrix}
	8 \\
	20 \\
	16
\end{bmatrix}
$$

$$
\left \downarrow
\begin{aligned}
	R_2 = R_2 - 2 R_1 \\
	R_3 = R_3 - 4 R_1
\end{aligned}
\right.
$$

$$
\begin{bmatrix}
	1 & 2 & 1 \\
	0 & -1 & 2 \\
	0 & -5 & -2
\end{bmatrix}
\begin{bmatrix}
	x \\
	y \\
	z
\end{bmatrix}
=
\begin{bmatrix}
	8 \\
	4 \\
	-16
\end{bmatrix}
$$

$$
\left \downarrow
\begin{aligned}
	R_3 = R_3 - 5 R_1 \\
\end{aligned}
\right.
$$

$$
\begin{bmatrix}
	1 & 0 & 5 \\
	0 & -1 & 2 \\
	0 & 0 & -12
\end{bmatrix}
\begin{bmatrix}
	x \\
	y \\
	z
\end{bmatrix}
=
\begin{bmatrix}
	16 \\
	4 \\
	-36
\end{bmatrix}
$$

$$
\left \downarrow
\begin{aligned}
	R_3 = \frac {R_3} {-12} \\
\end{aligned}
\right.
$$

$$
\begin{bmatrix}
	1 & 0 & 5 \\
	0 & -1 & 2 \\
	0 & 0 & 1
\end{bmatrix}
\begin{bmatrix}
	x \\
	y \\
	z
\end{bmatrix}
=
\begin{bmatrix}
	16 \\
	4 \\
	3
\end{bmatrix}
$$

$$
\left \downarrow
\begin{aligned}
	R_1 = R_1 - 5 R_3 \\
	R_2 = R_2 - 2 R_3 \\
\end{aligned}
\right.
$$

$$\begin{bmatrix}
	1 & 0 & 0 \\
	0 & -1 & 0 \\
	0 & 0 & 1
\end{bmatrix}
\begin{bmatrix}
	x \\
	y \\
	z
\end{bmatrix}
=
\begin{bmatrix}
	1 \\
	-2 \\
	3
\end{bmatrix}
$$

The solution is $(1, 2, 3)$.

## Crout’s Reduction Method

In this method, the `coefficient matrix`[^2] $A$ is decomposed as following

$$LU = A$$

$$
\begin{bmatrix}
	l_{11} & 0 & 0 \\
	l_{21} & l_{22} & 0 \\
	l_{31} & l_{32} & l_{33}
\end{bmatrix}
\begin{bmatrix}
	1 & u_{12} & u_{13} \\
	0 & 1 & u_{23} \\
	0 & 0 & 1
\end{bmatrix}
=
\begin{bmatrix}
	a_{11} & a_{12} & a_{13} \\
	a_{21} & a_{22} & a_{23} \\
	a_{31} & a_{32} & a_{33}
\end{bmatrix}
$$

### Step 1

Multiply all rows of $L$ with first column of $U$.

$$l_{11} = a_{11}, \quad l_{21} = a_{21}, \quad l_{31} = a_{31}$$

### Step 2

Multiply 1st row of $L$ with 2nd and 3rd column of $U$.

$$l_{11}u_{12} = a_{12}, \quad l_{11}u_{13} = a_{13}$$

$$\Downarrow$$

$$u_{12} = \frac{a_{12}}{l_{11}}, \quad u_{13} = \frac{a_{13}}{l_{11}}$$

### Step 3

Multiply 2nd and 3rd rows of $L$ with 2nd column of $U$.

$$l_{21}u_{12} + l_{22} = a_{22}, \quad l_{31}u_{12} + l_{32} = a_{32}$$

$$\Downarrow$$

$$l_{22} = a_{22} - l_{21}u_{12}, \quad l_{32} = a_{32} - l_{31}u_{12}$$

### Step 4

Multiply 2nd row of $L$ with 3rd column of $U$.

$$l_{21}u_{13} + l_{22}u_{23} = a_{23}$$

$$\Downarrow$$

$$u_{23} = \frac{a_{23} - l_{21}u_{13}}{l_{22}}$$

### Step 5

Multiply 3rd row of $L$ with 3rd column of $U$.

$$l_{31}u_{13} + l_{32}u_{23} + l_{33} = a_{33}$$

$$\Downarrow$$

$$l_{33} = a_{33} - l_{33}u_{13} - l_{32}u_{23}$$

### Example

$$
\begin{align}
	5x_1 - 2x_2 + x_3 &= 4 \\
	7x_1 + x_2 - 5x_3 &= 8 \\
	3x_1 + 7x_2 + 4x_3 &= 10
\end{align}
$$

#### Solution

$$
\begin{bmatrix}
	l_{11} & 0 & 0 \\
	l_{21} & l_{22} & 0 \\
	l_{31} & l_{32} & l_{33}
\end{bmatrix}
\begin{bmatrix}
	1 & u_{12} & u_{13} \\
	0 & 1 & u_{23} \\
	0 & 0 & 1
\end{bmatrix}
=
\begin{bmatrix}
	5 & -2 & 1 \\
	7 & 1 & -5 \\
	3 & 7 & 4
\end{bmatrix}
$$

##### Step 1

$$l_{11} = 5, \quad l_{21} = 7, \quad l_{31} = 3$$

##### Step 2

$$l_{11}u_{12} = -2, \quad l_{11}u_{13} = 1$$

$$u_{12} = -\frac{2}{5}, u_{13} = \frac{1}{5}$$

##### Step 3

$$
\left.
\begin{aligned}
	l_{21}u_{12} + l_{22} &= 1 \quad \text{or} \quad l_{22} = 1 + \frac{14}{5} = \frac{19}{5} \\
	l_{31}u_{12} + l_{32} &= 7 \quad \text{or} \quad l_{32} = 7 + \frac{6}{5} = \frac{41}{5}
\end{aligned}
\right\}
$$

##### Step 4

$$l_{21}u_{13} + l_{22}u_{23} = -5$$

$$\frac{19}{5}u_{23} = -5 - \frac{7}{5}$$

$$u_{23} = -\frac{32}{19}$$

##### Step 5

$$l_{31}u_{13} + l_{32}u_{23} + l_{33} = 4$$

$$l_{33} = \frac{327}{19}$$

$$LUX = B$$

$$
\begin{bmatrix}
	5 & 0 & 0 \\
	7 & \frac{19}{5} & 0 \\
	3 & \frac{41}{5} & \frac{327}{19}
\end{bmatrix}
\begin{bmatrix}
	1 & -\frac{2}{5} & \frac{1}{5} \\
	0 & 1 & -\frac{32}{19} \\
	0 & 0 & 1
\end{bmatrix}
\begin{bmatrix}
	x_1 \\
	x_2 \\
	x_3
\end{bmatrix}
=
\begin{bmatrix}
	4 \\
	8 \\
	10
\end{bmatrix}
$$

Substitute $UX = Z$.

$$
\begin{bmatrix}
	5 & 0 & 0 \\
	7 & \frac{19}{5} & 0 \\
	3 & \frac{41}{5} & \frac{327}{19}
\end{bmatrix}
\begin{bmatrix}
	z_1 \\
	z_2 \\
	z_3
\end{bmatrix} = \begin{bmatrix}
	4 \\
	8 \\
	10
\end{bmatrix}
$$

By using `back subsitution.

$$x_3 = \frac{46}{327}, \quad x_2 = \frac{284}{327}, \quad x_1 = \frac{366}{327}$$

## References

Read more about [[M_Notations|notations and symbols]].

[^1]: Read more about [[mth603_09|gaussian elimination method]].
[^2]: Read more about [[mth501_03|linear systems and coefficient matrices]].
[^3]: Read more about [[mth501_11|diagonal matrices]].